src3.0/Vellvm/Dominators/dom_type.v
@@ -1,13 +1,150 @@
+Require Import List.
+Require Import ListSet.
+Require Import Coqlib.
 Require Import Metatheory.
+Require Import Maps.
+Require Import Lattice.
 Require Import Kildall.
+Require Import Iteration.
+Require Import cfg.
+Require Import reach.
+Require Import Dipaths.
 
-Module Dom_Kildall.
+Require Import syntax.
+Require Import infrastructure.
+Require Import infrastructure_props.
+Import LLVMsyntax.
+Import LLVMinfra.
 
-Module DomDS := Dataflow_Solver_Var_Top(AtomNodeSet).
+Module Type ALGDOM.
 
-Section A.
+Parameter dom_analysis_is_successful : fdef -> Prop.
 
-End A.
+Parameter dom_query : fdef -> atom -> set atom.
 
-End Dom_Kildall.
+Axiom dom_entrypoint : forall f l0 ps cs tmn
+  (Hentry : getEntryBlock f = Some (block_intro l0 ps cs tmn)),
+  dom_query f l0 = nil.
+
+Definition wf_entrypoints f: Prop :=
+  match getEntryBlock f with
+  | Some (block_intro l0 _ _ _) => 
+      (XATree.make_predecessors (successors f))!!!l0 = nil
+  | _ => False
+  end.
+
+Axiom entry_doms_others: forall (f:fdef)
+  (Hwf_entrypoints: wf_entrypoints f) entry
+  (Hex: dom_analysis_is_successful f)
+  (H: getEntryLabel f = Some entry),
+  (forall b (H0: b <> entry /\ reachable f b),
+     ListSet.set_In entry (dom_query f b)).
+
+Axiom dom_query_in_bound: forall fh bs l5, 
+  incl (dom_query (fdef_intro fh bs) l5) (bound_blocks bs).
+
+Axiom dom_successors : forall
+  (l3 : l) (l' : l) f
+  (contents3 contents': ListSet.set atom)
+  (Hinscs : In l' (successors f) !!! l3)
+  (Heqdefs3 : contents3 = dom_query f l3)
+  (Heqdefs' : contents' = dom_query f l'),
+  incl contents' (l3 :: contents3).
+
+Axiom sdom_is_complete: forall (f:fdef)
+  (Hwf_entrypoints: wf_entrypoints f)
+  (branches_in_vertexes: forall p ps0 cs0 tmn0 l2
+    (J3 : blockInFdefB (block_intro p ps0 cs0 tmn0) f)
+    (J4 : In l2 (successors_terminator tmn0)),
+    vertexes_fdef f (index l2))
+  (l3 : l) (l' : l) ps cs tmn ps' cs' tmn'
+  (HuniqF : uniqFdef f)
+  (Hsucc: dom_analysis_is_successful f)
+  (HBinF' : blockInFdefB (block_intro l' ps' cs' tmn') f = true)
+  (HBinF : blockInFdefB (block_intro l3 ps cs tmn) f = true)
+  (Hsdom: strict_domination f l' l3),
+  In l' (dom_query f l3).
+
+Axiom dom_unreachable: forall (f:fdef)
+  (branches_in_vertexes: forall p ps0 cs0 tmn0 l2
+    (J3 : blockInFdefB (block_intro p ps0 cs0 tmn0) f)
+    (J4 : In l2 (successors_terminator tmn0)),
+    vertexes_fdef f (index l2))
+  (wf_entrypoints: wf_entrypoints f)
+  (l3 : l) (l' : l) ps cs tmn
+  (Hsucc: dom_analysis_is_successful f)
+  (HuniqF: uniqFdef f)
+  (HBinF : blockInFdefB (block_intro l3 ps cs tmn) f = true)
+  (Hunreach: ~ reachable f l3),
+  dom_query f l3 = bound_fdef f.
+
+Axiom dom_is_sound : forall (f : fdef)
+  (Hhasentry: getEntryBlock f <> None)
+  (l3 : l) (l' : l) ps cs tmn
+  (HBinF : blockInFdefB (block_intro l3 ps cs tmn) f = true)
+  (Hin : In l' (l3::(dom_query f l3))),
+  domination f l' l3.
+
+Axiom sdom_is_sound : forall (f : fdef)
+  (Hhasentry: getEntryBlock f <> None)
+  (l3 : l) (l' : l) ps cs tmn
+  (Hreach : reachable f l3)
+  (HBinF : blockInFdefB (block_intro l3 ps cs tmn) f = true)
+  (Hin : In l' (dom_query f l3)),
+  strict_domination f l' l3.
+
+Axiom sdom_isnt_refl : forall (f : fdef)
+  (Hhasentry: getEntryBlock f <> None)
+  (l3 : l) (l' : l) ps cs tmn
+  (Hreach : reachable f l3)
+  (HBinF : blockInFdefB (block_intro l3 ps cs tmn) f = true)
+  (Hin : In l' (dom_query f l3)),
+  l' <> l3.
+
+Definition getEntryBlock_inv f := forall
+  (l3 : l) (l' : l)
+  (ps : phinodes)
+  (cs : cmds)
+  (tmn : terminator)
+  (HBinF : blockInFdefB (block_intro l3 ps cs tmn) f = true)
+  (Hsucc : In l' (successors_terminator tmn)) a ps0 cs0 tmn0
+  (H : getEntryBlock f = Some (block_intro a ps0 cs0 tmn0)),
+  l' <> a.
+
+Axiom adom_acyclic: forall f 
+  (Hhasentry: getEntryBlock f <> None)
+  (HgetEntryBlock_inv : getEntryBlock_inv f)
+  l1 l2 ps1 cs1 tmn1 ps2 cs2 tmn2,
+  reachable f l2 ->
+  blockInFdefB (block_intro l1 ps1 cs1 tmn1) f = true ->
+  blockInFdefB (block_intro l2 ps2 cs2 tmn2) f = true ->
+  In l1 (dom_query f l2) ->
+  In l2 (dom_query f l1) ->
+  l1 <> l2 ->
+  False.
+
+Axiom pres_dom_query: forall 
+  (ftrans: fdef -> fdef) 
+  (btrans: block -> block)
+  (ftrans_spec: forall fh bs, 
+    ftrans (fdef_intro fh bs) = fdef_intro fh (List.map btrans bs))
+  (btrans_eq_label: forall b, getBlockLabel b = getBlockLabel (btrans b))
+  (btrans_eq_tmn: forall b, 
+    terminator_match (getBlockTmn b) (getBlockTmn (btrans b)))
+  (f : fdef) (l5 l0 : l),
+  ListSet.set_In l5 (dom_query f l0) <->
+  ListSet.set_In l5 (dom_query (ftrans f) l0).
+
+Axiom pres_dom_analysis_is_successful : forall 
+  (ftrans: fdef -> fdef) 
+  (btrans: block -> block)
+  (ftrans_spec: forall fh bs, 
+    ftrans (fdef_intro fh bs) = fdef_intro fh (List.map btrans bs))
+  (btrans_eq_label: forall b, getBlockLabel b = getBlockLabel (btrans b))
+  (btrans_eq_tmn: forall b, 
+    terminator_match (getBlockTmn b) (getBlockTmn (btrans b))) f,
+  dom_analysis_is_successful f <-> 
+    dom_analysis_is_successful (ftrans f).
+
+End ALGDOM.
 
