src3.0/Transforms/dtree_props.v
@@ -64,14 +64,23 @@ Ltac solve_in_dec :=
       destruct (in_dec dec a s); auto
   end.
 
+Ltac elim_in_nil :=
+match goal with
+| i0: In _ ?l |- ?l <> nil =>
+  let J := fresh "J" in
+  intro J; rewrite J in i0; auto
+| i0: In _ ?l, H: ?l = nil |- False =>
+  rewrite H in i0; auto
+end.
+
 Lemma gt_dom_prop_trans : forall S M f l1 l2 l3
   (HwfF: wf_fdef S M f) (Huniq: uniqFdef f)
   (HBinF1: In l1 (bound_fdef f))
   (HBinF2: In l2 (bound_fdef f))
   (HBinF3: In l3 (bound_fdef f))
-  (H1 : gt_dom_prop (bound_fdef f) (dom_analyze f) l1 l2)
-  (H2 : gt_dom_prop (bound_fdef f) (dom_analyze f)  l2 l3),
-  gt_dom_prop (bound_fdef f) (dom_analyze f) l1 l3.
+  (H1 : gt_dom_prop (AlgDom.dom_query f) l1 l2)
+  (H2 : gt_dom_prop (AlgDom.dom_query f) l2 l3),
+  gt_dom_prop (AlgDom.dom_query f) l1 l3.
 Proof.
   unfold gt_dom_prop, gt_sdom.
   intros.
@@ -95,17 +104,17 @@ Proof.
         eapply dom_is_sound; simpl; eauto.
       assert (strict_domination f l1 l3) as Hsdom13.
         split; auto.
-          eapply dom_tran; eauto.
+          eapply DecDom.dom_tran; eauto.
       eapply sdom_is_complete in Hsdom13; eauto 1.
         solve_in_dec.
-        intro J. unfold dom_query in J. rewrite J in i0. auto.
+        elim_in_nil.
 
     SCase "l1=l2".
       assert (strict_domination f l2 l3) as Hsdom23.
         split; auto.
       eapply sdom_is_complete in Hsdom23; eauto 1.
         solve_in_dec.
-        intro J. unfold dom_query in J. rewrite J in i0. auto.
+        elim_in_nil.
 Qed.
 
 Lemma gt_sdom_prop_trans : forall S M f l1 l2 l3
@@ -113,9 +122,9 @@ Lemma gt_sdom_prop_trans : forall S M f l1 l2 l3
   (HBinF1: In l1 (bound_fdef f))
   (HBinF2: In l2 (bound_fdef f))
   (HBinF3: In l3 (bound_fdef f))
-  (H1 : gt_sdom (bound_fdef f) (dom_analyze f) l1 l2 = true)
-  (H2 : gt_sdom (bound_fdef f) (dom_analyze f)  l2 l3 = true),
-  gt_sdom (bound_fdef f) (dom_analyze f)  l1 l3 = true.
+  (H1 : gt_sdom (AlgDom.dom_query f) l1 l2 = true)
+  (H2 : gt_sdom (AlgDom.dom_query f)  l2 l3 = true),
+  gt_sdom (AlgDom.dom_query f)  l1 l3 = true.
 Proof.
   unfold gt_sdom.
   intros.
@@ -130,50 +139,23 @@ Proof.
     assert (strict_domination f l2 l3) as Hsdom23.
       eapply sdom_is_sound; eauto.
     assert (reachable f l2) as Hreach2.
-      apply sdom_reachable in Hsdom23; auto.
+      apply DecDom.sdom_reachable in Hsdom23; auto.
     assert (strict_domination f l1 l2) as Hsdom12.
       eapply sdom_is_sound; eauto.
     assert (strict_domination f l1 l3) as Hsdom13.
       eapply sdom_tran with (l2:=l2); eauto.
     eapply sdom_is_complete in Hsdom13; eauto 1.
       solve_in_dec.
-      intro J. unfold dom_query in J. rewrite J in i0. auto.
+      elim_in_nil.
 
     eapply dom_unreachable in H; eauto 1.
       apply blockInFdefB_in_vertexes in HBinF1.
       unfold vertexes_fdef in HBinF1.
-      destruct ((dom_analyze f) !! l3); tinv H; simpl.
+      rewrite H.
       solve_in_dec.
 
-      intro J. unfold dom_query in J. rewrite J in i0. auto.
+      elim_in_nil.
 Qed.
-
-(*
-Lemma sdom_ordered : forall f l1 l2 l3
-  (Hneq: l1 <> l2) (Hreach: reachable f l3)
-  (Hsdom: strict_domination f l1 l3)
-  (Hsdom': strict_domination f l2 l3),
-  strict_domination f l1 l2 \/ strict_domination f l2 l1.
-
-Lemma sdom_is_sound : forall
-  ifs S M (f : fdef) (l3 : l) (l' : l) ps cs tmn
-  (HwfF : wf_fdef ifs S M f) (HuniqF : uniqFdef f) (Hreach : reachable f l3)
-  (HBinF : blockInFdefB (block_intro l3 ps cs tmn) f = true)
-  (Hin :
-    In l' (DomDS.L.bs_contents _ ((dom_analyze f) !! l3))),
-  strict_domination f l' l3.
-Proof.
-Lemma sdom_is_complete: forall
-  ifs S M (f : fdef) (l3 : l) (l' : l) ps cs tmn ps' cs' tmn'
-  (HwfF : wf_fdef ifs S M f) (HuniqF : uniqFdef f)
-  (HBinF' : blockInFdefB (block_intro l' ps' cs' tmn') f = true)
-  (HBinF : blockInFdefB (block_intro l3 ps cs tmn) f = true)
-  (Hsdom: strict_domination f l' l3)
-  (Hnempty: DomDS.L.bs_contents _ ((dom_analyze f) !! l3) <> nil),
-  In l' (DomDS.L.bs_contents _ ((dom_analyze f) !! l3)).
-Proof.
-
-*)
 
 Lemma gt_dom_dec_aux: forall S M f (HwfF: wf_fdef S M f) 
   (Huniq: uniqFdef f) l1 l2 l3
@@ -181,10 +163,10 @@ Lemma gt_dom_dec_aux: forall S M f (HwfF: wf_fdef S M f)
   (HBinF1: In l1 (bound_fdef f))
   (HBinF2: In l2 (bound_fdef f))
   (HBinF3: In l3 (bound_fdef f)),
-  gt_sdom (bound_fdef f) (dom_analyze f) l1 l3 ->
-  gt_sdom (bound_fdef f) (dom_analyze f) l2 l3 ->
-  gt_dom_prop (bound_fdef f) (dom_analyze f) l1 l2 \/
-  gt_dom_prop (bound_fdef f) (dom_analyze f) l2 l1.
+  gt_sdom (AlgDom.dom_query f) l1 l3 ->
+  gt_sdom (AlgDom.dom_query f) l2 l3 ->
+  gt_dom_prop (AlgDom.dom_query f) l1 l2 \/
+  gt_dom_prop (AlgDom.dom_query f) l2 l1.
 Proof.
   unfold gt_dom_prop, gt_sdom. intros.
   destruct (l_dec l1 l2); auto.
@@ -208,26 +190,26 @@ Proof.
     end.
   destruct Hentry as [entry Hentry].
   assert (reachable f l2) as Hreach2.
-    apply sdom_reachable in Hsdom23; auto.
+    apply DecDom.sdom_reachable in Hsdom23; auto.
   assert (reachable f l1) as Hreach1.
-    apply sdom_reachable in Hsdom13; auto.
+    apply DecDom.sdom_reachable in Hsdom13; auto.
   destruct (l_dec l1 entry); subst.
     left. left.
-    assert (set_In entry (dom_query f l2)) as G.
+    assert (set_In entry (AlgDom.dom_query f l2)) as G.
       eapply dom_analysis__entry_doms_others; eauto.
     solve_in_dec.
   destruct (l_dec l2 entry); subst.
     right. left.
-    assert (set_In entry (dom_query f l1)) as G.
+    assert (set_In entry (AlgDom.dom_query f l1)) as G.
       eapply dom_analysis__entry_doms_others; eauto.
     solve_in_dec.
-  eapply sdom_ordered with (l1:=l2) in Hsdom13; eauto 1.
+  eapply DecDom.sdom_ordered with (l1:=l2) in Hsdom13; eauto 1.
   destruct Hsdom13 as [Hsdom21 | Hsdom12].
     right.
     eapply sdom_is_complete in Hsdom21; eauto 1.
       left. solve_in_dec.
 
-      assert (set_In entry (dom_query f l1)) as G.
+      assert (set_In entry (AlgDom.dom_query f l1)) as G.
         eapply dom_analysis__entry_doms_others; eauto.
       intro J. rewrite J in G. auto.
 
@@ -235,7 +217,7 @@ Proof.
     eapply sdom_is_complete in Hsdom12; eauto 1.
       left. solve_in_dec.
 
-      assert (set_In entry (dom_query f l2)) as G.
+      assert (set_In entry (AlgDom.dom_query f l2)) as G.
         eapply dom_analysis__entry_doms_others; eauto.
       intro J. rewrite J in G. auto.
 Qed.
@@ -246,10 +228,10 @@ Lemma gt_dom_dec: forall S M f (HwfF: wf_fdef S M f)
   (HBinF1: In l1 (bound_fdef f))
   (HBinF2: In l2 (bound_fdef f))
   (HBinF3: In l3 (bound_fdef f)),
-  gt_dom_prop (bound_fdef f) (dom_analyze f) l1 l3 ->
-  gt_dom_prop (bound_fdef f) (dom_analyze f) l2 l3 ->
-  gt_dom_prop (bound_fdef f) (dom_analyze f) l1 l2 \/
-  gt_dom_prop (bound_fdef f) (dom_analyze f) l2 l1.
+  gt_dom_prop (AlgDom.dom_query f) l1 l3 ->
+  gt_dom_prop (AlgDom.dom_query f) l2 l3 ->
+  gt_dom_prop (AlgDom.dom_query f) l1 l2 \/
+  gt_dom_prop (AlgDom.dom_query f) l2 l1.
 Proof.
   intros.
   destruct H as [H | H]; subst; auto.
@@ -265,10 +247,10 @@ Lemma gt_sdom_dec: forall S M f (HwfF: wf_fdef S M f)
   (HBinF1: In l1 (bound_fdef f))
   (HBinF2: In l2 (bound_fdef f))
   (HBinF3: In l3 (bound_fdef f)),
-  gt_sdom (bound_fdef f) (dom_analyze f) l1 l3 ->
-  gt_sdom (bound_fdef f) (dom_analyze f) l2 l3 ->
-  gt_sdom (bound_fdef f) (dom_analyze f) l1 l2 \/
-  gt_sdom (bound_fdef f) (dom_analyze f) l2 l1.
+  gt_sdom (AlgDom.dom_query f) l1 l3 ->
+  gt_sdom (AlgDom.dom_query f) l2 l3 ->
+  gt_sdom (AlgDom.dom_query f) l1 l2 \/
+  gt_sdom (AlgDom.dom_query f) l2 l1.
 Proof.
   intros.
   apply gt_dom_dec with (l1:=l1) (l2:=l2) (l3:=l3) in HwfF; auto.
@@ -277,9 +259,9 @@ Proof.
     left. auto.
 Qed.
 
-Lemma insert_sort_sdom_iter_safe: forall bd res l0 suffix l1 prefix,
+Lemma insert_sort_sdom_iter_safe: forall res l0 suffix l1 prefix,
   (In l0 (prefix ++ suffix) \/ l0 = l1) <->
-  In l0 (insert_sort_sdom_iter bd res l1 prefix suffix).
+  In l0 (insert_sort_sdom_iter res l1 prefix suffix).
 Proof.
   induction suffix; simpl; intros.
     split; intro J.
@@ -295,7 +277,7 @@ Proof.
 
     simpl_env. simpl.
     split; intro J.
-      destruct (gt_sdom bd res l1 a).
+      destruct (gt_sdom res l1 a).
         destruct J as [J | J]; subst.
           apply in_app_or in J. simpl in J.
           apply in_or_app. simpl.
@@ -311,7 +293,7 @@ Proof.
             right. apply in_or_app; auto.
             right. apply in_or_app; auto.
 
-      destruct (gt_sdom bd res l1 a).
+      destruct (gt_sdom res l1 a).
         apply in_app_or in J. simpl in J.
         destruct J as [J | [J | [J | J]]]; subst; auto.
           left. apply in_or_app. simpl.
@@ -326,8 +308,8 @@ Proof.
           destruct J as [[J | J] | J]; subst; auto.
 Qed.
 
-Lemma insert_sort_sdom_safe: forall bd res data acc l0,
-  (In l0 acc \/ In l0 data) <-> In l0 (insert_sort_sdom bd res data acc).
+Lemma insert_sort_sdom_safe: forall res data acc l0,
+  (In l0 acc \/ In l0 data) <-> In l0 (insert_sort_sdom res data acc).
 Proof.
   induction data; simpl; intros; auto.
     split; tauto.
@@ -347,12 +329,12 @@ Proof.
       destruct H; auto.
 Qed.
 
-Lemma sort_sdom_safe: forall bd res input l0,
-  In l0 (sort_sdom bd res input) <-> In l0 input.
+Lemma sort_sdom_safe: forall res input l0,
+  In l0 (sort_sdom res input) <-> In l0 input.
 Proof.
   intros.
   unfold sort_sdom.
-  destruct (@insert_sort_sdom_safe bd res input nil l0) as [J1 J2].
+  destruct (@insert_sort_sdom_safe res input nil l0) as [J1 J2].
   split; intro; auto.
     apply J2 in H. destruct H as [H | H]; auto. inv H.
 Qed.
@@ -360,15 +342,15 @@ Qed.
 Lemma insert_sort_sdom_iter_sorted: forall S M f (HwfF: wf_fdef S M f) 
   (Huniq: uniqFdef f) l3 (Hin3: In l3 (bound_fdef f)) (Hreach: reachable f l3)
   l0 (Hin0: In l0 (bound_fdef f))
-  (Hsd03: gt_dom_prop (bound_fdef f) (dom_analyze f) l0 l3) suffix prefix
+  (Hsd03: gt_dom_prop (AlgDom.dom_query f) l0 l3) suffix prefix
   (G: forall l', In l' (prefix ++ suffix) ->
-      gt_dom_prop (bound_fdef f) (dom_analyze f) l' l3 /\ In l' (bound_fdef f)),
-  Sorted (gt_dom_prop (bound_fdef f) (dom_analyze f))
+      gt_dom_prop (AlgDom.dom_query f) l' l3 /\ In l' (bound_fdef f)),
+  Sorted (gt_dom_prop (AlgDom.dom_query f))
     (List.rev prefix ++ suffix) ->
   (forall l1 prefix', prefix = l1 :: prefix' ->
-      gt_dom_prop (bound_fdef f) (dom_analyze f) l1 l0) ->
-  Sorted (gt_dom_prop (bound_fdef f) (dom_analyze f))
-    (insert_sort_sdom_iter (bound_fdef f) (dom_analyze f) l0 prefix suffix).
+      gt_dom_prop (AlgDom.dom_query f) l1 l0) ->
+  Sorted (gt_dom_prop (AlgDom.dom_query f))
+    (insert_sort_sdom_iter (AlgDom.dom_query f) l0 prefix suffix).
 Proof.
   induction suffix; simpl; intros.
     simpl_env in *.
@@ -378,7 +360,7 @@ Proof.
         rewrite <- rev_involutive at 1.
         rewrite H1. rewrite rev_unit. auto.
 
-    remember (gt_sdom (bound_fdef f) (dom_analyze f) l0 a) as R.
+    remember (gt_sdom (AlgDom.dom_query f) l0 a) as R.
     destruct R.
       simpl_env. simpl.
       apply sorted_insert; auto.
@@ -400,8 +382,8 @@ Proof.
         simpl. simpl_env. simpl. auto.
 
         intros. inv H1.
-        assert (gt_dom_prop (bound_fdef f) (dom_analyze f) l1 l0 \/
-                gt_dom_prop (bound_fdef f) (dom_analyze f) l0 l1) as J.
+        assert (gt_dom_prop (AlgDom.dom_query f) l1 l0 \/
+                gt_dom_prop (AlgDom.dom_query f) l0 l1) as J.
           assert (In l1 (prefix'++l1::suffix)) as Hin1. apply in_middle.
           apply G in Hin1. destruct Hin1 as [J1 J2].
           eapply gt_dom_dec; eauto.
@@ -416,10 +398,10 @@ Lemma insert_sort_sdom_sorted: forall S M f (HwfF: wf_fdef S M f)
   (Huniq: uniqFdef f) l3 (Hin3: In l3 (bound_fdef f)) (Hreach: reachable f l3)
   data acc
   (G: forall l', In l' (data++acc) ->
-      gt_dom_prop (bound_fdef f) (dom_analyze f) l' l3 /\ In l' (bound_fdef f)),
-  Sorted (gt_dom_prop (bound_fdef f) (dom_analyze f)) acc ->
-  Sorted (gt_dom_prop (bound_fdef f) (dom_analyze f))
-         (insert_sort_sdom (bound_fdef f) (dom_analyze f) data acc).
+      gt_dom_prop (AlgDom.dom_query f) l' l3 /\ In l' (bound_fdef f)),
+  Sorted (gt_dom_prop (AlgDom.dom_query f)) acc ->
+  Sorted (gt_dom_prop (AlgDom.dom_query f))
+         (insert_sort_sdom (AlgDom.dom_query f) data acc).
 Proof.
   induction data; simpl; intros; auto.
     apply IHdata.
@@ -443,9 +425,9 @@ Lemma sort_sdom_sorted: forall S M f (HwfF: wf_fdef S M f)
   (Huniq: uniqFdef f) l3 (Hin3: In l3 (bound_fdef f)) (Hreach: reachable f l3)
   input
   (G: forall l', In l' input ->
-      gt_dom_prop (bound_fdef f) (dom_analyze f) l' l3 /\ In l' (bound_fdef f)),
-  Sorted (gt_dom_prop (bound_fdef f) (dom_analyze f))
-         (sort_sdom (bound_fdef f) (dom_analyze f) input).
+      gt_dom_prop (AlgDom.dom_query f) l' l3 /\ In l' (bound_fdef f)),
+  Sorted (gt_dom_prop (AlgDom.dom_query f))
+         (sort_sdom (AlgDom.dom_query f) input).
 Proof.
   intros. unfold sort_sdom.
   eapply insert_sort_sdom_sorted; simpl_env; eauto.
@@ -569,7 +551,7 @@ Qed.
 
 Lemma gt_sdom_prop_irrefl: forall S M f (HwfF : wf_fdef S M f) 
   (HuniqF: uniqFdef f) a (Hreach : reachable f a),
-  gt_sdom (bound_fdef f) (dom_analyze f) a a = false.
+  gt_sdom (AlgDom.dom_query f) a a = false.
 Proof.
   unfold gt_sdom.
   intros.
@@ -577,8 +559,7 @@ Proof.
   apply reachable__in_bound in Hreach.
   apply In_bound_fdef__blockInFdefB in Hreach.
   destruct Hreach as [ps [cs [tnn HBinF]]].
-  destruct (in_dec l_dec a 
-    (bound_dom (bound_fdef f) (dom_analyze f) !! a)); simpl; auto.
+  destruct (in_dec l_dec a (AlgDom.dom_query f a)); simpl; auto.
   eapply sdom_is_sound with (l':=a) in HBinF; eauto 1.
     destruct HBinF. congruence.
 Qed.
@@ -621,8 +602,8 @@ Proof.
       apply Sorted_HdRel__Forall in H; auto.
 Qed.
 
-Lemma compute_sdom_chains_aux__dom : forall bd res l0 chain0 rd acc,
-  In (l0, chain0) (compute_sdom_chains_aux bd res rd acc) ->
+Lemma compute_sdom_chains_aux__dom : forall res l0 chain0 rd acc,
+  In (l0, chain0) (compute_sdom_chains_aux res rd acc) ->
   In l0 rd \/ In (l0, chain0) acc.
 Proof.
   induction rd; simpl; intros; auto.
@@ -633,8 +614,8 @@ Proof.
     inv H; auto.
 Qed.
 
-Lemma compute_sdom_chains__dom : forall bd res rd l0 chain0,
-  In (l0, chain0) (compute_sdom_chains bd res rd) -> In l0 rd.
+Lemma compute_sdom_chains__dom : forall res rd l0 chain0,
+  In (l0, chain0) (compute_sdom_chains res rd) -> In l0 rd.
 Proof.
   unfold compute_sdom_chains.
   intros.
@@ -645,7 +626,7 @@ Qed.
 
 Lemma compute_sdom_chains_aux_sorted__helper: forall bd0 bd bs_contents res x
   (bs_bound : incl bs_contents bd0) (l1 : l) (Hinc : incl (l1 :: bd) bd0)
-  (H1 : In x (sort_sdom bd0 res (l1 :: bs_contents))),
+  (H1 : In x (sort_sdom res (l1 :: bs_contents))),
   In x bd0.
 Proof.
   intros.
@@ -656,8 +637,15 @@ Proof.
     apply bs_bound. auto.
 Qed.
 
+Lemma in_bound_dom__in_bound_fdef: forall l' f l1
+  (Hin: In l' (AlgDom.dom_query f l1)),
+  In l' (bound_fdef f).
+Proof.
+  intros. destruct f. eapply AlgDom.dom_query_in_bound; eauto.
+Qed.
+
 Lemma in_gt_sdom__in_bound_fdef: forall f l1 l2
-  (Hin: gt_sdom (bound_fdef f) (dom_analyze f) l1 l2 = true),
+  (Hin: gt_sdom (AlgDom.dom_query f) l1 l2 = true),
   In l1 (bound_fdef f).
 Proof.
   unfold gt_sdom.
@@ -668,9 +656,9 @@ Qed.
 Lemma gt_sdom_prop_trans1 : forall S M f l1 l2 l3
   (HwfF: wf_fdef S M f) (Huniq: uniqFdef f) (Hreach: reachable f l3)
   (HBinF2: In l2 (bound_fdef f))
-  (H1 : gt_sdom (bound_fdef f) (dom_analyze f) l1 l2 = true)
-  (H2 : gt_dom_prop (bound_fdef f) (dom_analyze f) l2 l3),
-  gt_sdom (bound_fdef f) (dom_analyze f) l1 l3 = true.
+  (H1 : gt_sdom (AlgDom.dom_query f) l1 l2 = true)
+  (H2 : gt_dom_prop (AlgDom.dom_query f) l2 l3),
+  gt_sdom (AlgDom.dom_query f) l1 l3 = true.
 Proof.
   intros.
   assert (HBinF1: In l1 (bound_fdef f)).
@@ -690,7 +678,7 @@ Proof.
       destruct H2 as [H2 | H2]; simpl; auto.
         simpl_in_dec; auto.
   assert (reachable f l2) as Hreach2.
-     apply dom_reachable in Hdom23; auto.
+     apply DecDom.dom_reachable in Hdom23; auto.
   assert (strict_domination f l1 l2) as Hsdom12.
     eapply sdom_is_sound; eauto.
   eapply sdom_tran1 with (l3:=l3) in Hsdom12; eauto 1.
@@ -699,9 +687,9 @@ Proof.
 
     destruct H2 as [H2 | H2]; subst.
       simpl_in_dec.
-      intro J. unfold dom_query in J. rewrite J in i1. auto.
+      elim_in_nil.
 
-      intro J. unfold dom_query in J. rewrite J in i0. auto.
+      elim_in_nil.
 Qed.
 
 Lemma compute_sdom_chains_aux_sorted: forall S M f 
@@ -709,11 +697,11 @@ Lemma compute_sdom_chains_aux_sorted: forall S M f
   l0 chain0 bd (Hinc: incl bd (bound_fdef f))
   (Hreach: forall x, In x bd -> reachable f x) acc,
   (forall l0 chain0, In (l0, chain0) acc ->
-    Sorted (gt_dom_prop (bound_fdef f) (dom_analyze f)) chain0 /\
+    Sorted (gt_dom_prop (AlgDom.dom_query f)) chain0 /\
     NoDup chain0) ->
   In (l0, chain0)
-    (compute_sdom_chains_aux (bound_fdef f) (dom_analyze f) bd acc) ->
-  Sorted (gt_dom_prop (bound_fdef f) (dom_analyze f)) chain0 /\ NoDup chain0.
+    (compute_sdom_chains_aux (AlgDom.dom_query f) bd acc) ->
+  Sorted (gt_dom_prop (AlgDom.dom_query f)) chain0 /\ NoDup chain0.
 Proof.
   induction bd as [|a bd]; simpl; intros; eauto.
     apply IHbd in H0; auto.
@@ -727,8 +715,8 @@ Proof.
       assert (In l1 (bound_fdef f)) as G1.
         apply Hinc; simpl; auto.
       assert (forall l' : l,
-        In l' (l1 :: bound_dom (bound_fdef f) ((dom_analyze f) !! l1)) ->
-        gt_dom_prop (bound_fdef f) (dom_analyze f) l' l1 /\ In l' (bound_fdef f))
+        In l' (l1 :: AlgDom.dom_query f l1) ->
+        gt_dom_prop (AlgDom.dom_query f) l' l1 /\ In l' (bound_fdef f))
         as G2.
         intros l' Hin.
         simpl in Hin.
@@ -746,7 +734,7 @@ Proof.
           eapply sort_sdom_sorted; eauto.
       SCase "2.2".
         apply remove_redundant_NoDup with
-          (R:=gt_dom_prop (bound_fdef f) (dom_analyze f)); auto.
+          (R:=gt_dom_prop (AlgDom.dom_query f)); auto.
         SSCase "2.2.1".
           intros.
           destruct H5; subst; try congruence.
@@ -757,7 +745,7 @@ Proof.
                 apply Hreach; auto.
 
                 assert (reachable f l1) as Hreach1. apply Hreach; auto.
-                eapply sdom_reachable; eauto.
+                eapply DecDom.sdom_reachable; eauto.
                   assert (In l1 (bound_fdef f)) as Hin.
                     apply Hinc; simpl; auto.
                   apply In_bound_fdef__blockInFdefB in Hin.
@@ -768,8 +756,8 @@ Ltac find_in_bound_fdef :=
 match goal with
 | G1 : In ?l1 (bound_fdef ?f),
   H2 : In ?b
-         (sort_sdom (bound_fdef ?f) (dom_analyze ?f)
-            (?l1 :: bound_dom (bound_fdef ?f) (dom_analyze ?f) !! ?l1)) |-
+         (sort_sdom (AlgDom.dom_query ?f)
+            (?l1 :: AlgDom.dom_query ?f ?l1)) |-
   In ?b (bound_fdef ?f) =>
   apply sort_sdom_safe in H2;
   destruct_in H2; eauto using in_bound_dom__in_bound_fdef
@@ -792,9 +780,9 @@ end.
 Qed.
 
 Lemma NoDup_gt_dom_prop_sorted__gt_dsom_prop_sorted: forall f chain
-  (Hsorted: Sorted (gt_dom_prop (bound_fdef f) (dom_analyze f)) chain)
+  (Hsorted: Sorted (gt_dom_prop (AlgDom.dom_query f)) chain)
   (Huniq: NoDup chain),
-  Sorted (gt_sdom_prop (bound_fdef f) (dom_analyze f)) chain.
+  Sorted (gt_sdom_prop (AlgDom.dom_query f)) chain.
 Proof.
   intros.
   induction Hsorted; simpl; intros; auto.
@@ -810,8 +798,8 @@ Lemma compute_sdom_chains_sorted: forall S M f
   (HwfF: wf_fdef S M f) (Huniq: uniqFdef f)
   rd (Hinc: incl rd (bound_fdef f)) (Hreach: forall x, In x rd -> reachable f x)
   l0 chain,
-  In (l0, chain) (compute_sdom_chains (bound_fdef f) (dom_analyze f) rd) ->
-  Sorted (gt_sdom_prop (bound_fdef f) (dom_analyze f)) chain /\ NoDup chain.
+  In (l0, chain) (compute_sdom_chains (AlgDom.dom_query f) rd) ->
+  Sorted (gt_sdom_prop (AlgDom.dom_query f)) chain /\ NoDup chain.
 Proof.
   intros.
   unfold compute_sdom_chains in H.
@@ -823,14 +811,14 @@ Proof.
     simpl. intros. tauto.
 Qed.
 
-Lemma compute_sdom_chains_aux_safe: forall bd0 (res:AMap.t Dominators.t)
+Lemma compute_sdom_chains_aux_safe: forall (res:l -> set l)
   l0 l1 chain0 dts0 bd acc,
   (forall l0 l1 chain0 dts0,
     In (l0, chain0) acc ->
-    bound_dom bd0 (AMap.get l0 res) = dts0 ->
+    res l0 = dts0 ->
     (In l1 chain0 <-> In l1 (l0 :: dts0))) ->
-  In (l0, chain0) (compute_sdom_chains_aux bd0 res bd acc) ->
-  bound_dom bd0 (AMap.get l0 res) = dts0 ->
+  In (l0, chain0) (compute_sdom_chains_aux res bd acc) ->
+  res l0 = dts0 ->
   (In l1 chain0 <-> In l1 (l0 :: dts0)).
 Proof.
   induction bd; intros; eauto.
@@ -839,17 +827,15 @@ Proof.
     intros. simpl in H2.
     destruct H2 as [H2 | H2]; eauto.
     inv H2. 
-    destruct (@remove_redundant_safe l3 
-                (sort_sdom bd0 res (l2 :: bound_dom bd0 res !! l2)))
+    destruct (@remove_redundant_safe l3 (sort_sdom res (l2 :: res l2)))
       as [J1 J2].
-    destruct (@sort_sdom_safe bd0 res (l2 :: 
-                 bound_dom bd0 res !! l2) l3) as [J3 J4].
+    destruct (@sort_sdom_safe res (l2 :: res l2) l3) as [J3 J4].
     split; eauto.
 Qed.
 
-Lemma compute_sdom_chains_safe: forall bd res rd l0 chain l1 dts0 ,
-  In (l0, chain) (compute_sdom_chains bd res rd) ->
-  bound_dom bd (AMap.get l0 res) = dts0 ->
+Lemma compute_sdom_chains_safe: forall res rd l0 chain l1 dts0 ,
+  In (l0, chain) (compute_sdom_chains res rd) ->
+  res l0 = dts0 ->
   (In l1 chain <-> In l1 (l0 :: dts0)).
 Proof.
   intros.
@@ -860,7 +846,7 @@ Qed.
 
 Lemma gt_sdom_prop_entry: forall f l1 entry
   (H: getEntryLabel f = ret entry)
-  (H4: gt_sdom_prop (bound_fdef f) (dom_analyze f) l1 entry),
+  (H4: gt_sdom_prop (AlgDom.dom_query f) l1 entry),
   False.
 Proof.
   intros.
@@ -870,17 +856,16 @@ Proof.
     destruct f as [fh bs]. destruct bs; tinv H.
     destruct b; inv H; simpl; eauto.
   destruct Hentry as [ps [cs [tmn Hentry]]].
-  apply dom_entrypoint in Hentry.
-  unfold dom_query in Hentry. rewrite Hentry in H4. 
-  simpl_in_dec. auto.
+  apply AlgDom.dom_entrypoint in Hentry.
+  simpl_in_dec. rewrite Hentry in i0. auto.
 Qed.
 
-Lemma entry_in_compute_sdom_chains: forall entry l0 chain0 bd res rd
+Lemma entry_in_compute_sdom_chains: forall entry l0 chain0 res rd
   (H:forall b, b <> entry /\ In b rd ->
-     match bound_dom bd (AMap.get b res) with
+     match res b with
      | dts => In entry dts
      end)
-  (H0:In (l0, chain0) (compute_sdom_chains bd res rd))
+  (H0:In (l0, chain0) (compute_sdom_chains res rd))
   (Huniq:NoDup chain0)
   (G:(length chain0 > 1)%nat),
   In entry chain0.
@@ -897,7 +882,7 @@ Qed.
 
 Lemma compute_sdom_chains__in_bound: forall l0 chain0 f rd
   (Hinc: incl rd (bound_fdef f)),
-  In (l0, chain0) (compute_sdom_chains (bound_fdef f) (dom_analyze f) rd) ->
+  In (l0, chain0) (compute_sdom_chains (AlgDom.dom_query f) rd) ->
   incl chain0 (bound_fdef f).
 Proof.
   intros.
@@ -916,14 +901,14 @@ Lemma entry_is_head_of_compute_sdom_chains: forall S M f
   (H:getEntryLabel f = Some entry)
   (H0:reachablity_analysis f = Some rd)
   (H1:In (l0, chain0)
-    (compute_sdom_chains (bound_fdef f) (dom_analyze f) rd))
+    (compute_sdom_chains (AlgDom.dom_query f) rd))
   (G:(length chain0 > 1)%nat),
   exists chain0', chain0 = entry :: chain0'.
 Proof.
   intros.
   assert (forall b,
     b <> entry /\ In b rd ->
-    match bound_dom (bound_fdef f) (AMap.get b (dom_analyze f)) with
+    match AlgDom.dom_query f b with
     | dts => In entry dts
     end) as J.
     intros b Hp.
@@ -963,7 +948,7 @@ Lemma compute_sdom_chains__wf_chain: forall S M f
   (HwfF: wf_fdef S M f) (Huniq: uniqFdef f) l0 chain0 entry rd,
   getEntryLabel f = Some entry ->
   reachablity_analysis f =  Some rd ->
-  In (l0, chain0) (compute_sdom_chains (bound_fdef f) (dom_analyze f) rd) ->
+  In (l0, chain0) (compute_sdom_chains (AlgDom.dom_query f) rd) ->
   wf_chain f (DT_node entry DT_nil) chain0.
 Proof.
   intros.
@@ -1398,9 +1383,8 @@ Lemma create_dtree__wf_dtree: forall f dt,
   create_dtree f = Some dt ->
   match getEntryLabel f, reachablity_analysis f with
   | Some root, Some rd =>
-      let dt' := dom_analyze f in
-      let b := bound_fdef f in
-      let chains := compute_sdom_chains b dt' rd in
+      let dt' := AlgDom.dom_query f in
+      let chains := compute_sdom_chains dt' rd in
       forall p0 ch0,
         (is_dtree_edge dt p0 ch0 ->
          exists l0, exists chain0,
@@ -1420,7 +1404,7 @@ Proof.
   destruct R; inv H.
   intros.
   destruct (@fold_left_create_dtree_from_chain__is_dtree_edge__is_chain_edge
-    p0 ch0 (compute_sdom_chains (bound_fdef f) (dom_analyze f) l1)
+    p0 ch0 (compute_sdom_chains (AlgDom.dom_query f) l1)
     (DT_node l0 DT_nil)) as [J1 J2].
   split; intros J; auto.
     apply J1 in J.
