src3.0/Transforms/filter.v
@@ -1373,7 +1373,7 @@ Proof.
   match goal with
   | Hentry : getEntryBlock _ = _,
     Hnpred : has_no_predecessors _ _ = _,
-    Hsuccess: dom_analysis_is_successful _ |- _ =>
+    Hsuccess: AlgDom.dom_analysis_is_successful _ |- _ =>
      eapply (@TransCFG.pres_getEntryBlock (Filter check))
        in Hentry; eauto;
      erewrite (@TransCFG.pres_has_no_predecessors (Filter check)) 
