src3.0/Transforms/mem2reg.v
@@ -510,8 +510,8 @@ match getEntryBlock f, reachablity_analysis f with
           (macro_mem2reg_fdef_step rd succs preds) (f0, nil) 
       else
         let b := bound_fdef f in
-        let dts := dom_analyze f in
-        let chains := compute_sdom_chains b dts rd in
+        let dts := AlgDom.dom_query f in
+        let chains := compute_sdom_chains dts rd in
         let dt :=
           fold_left
             (fun acc elt =>
