src3.0/Transforms/phiplacement_bsim_wfS.v
@@ -1350,7 +1350,7 @@ Proof.
   match goal with
   | Hentry : getEntryBlock _ = _,
     Hnpred : has_no_predecessors _ _ = _,
-    Hsuccess: dom_analysis_is_successful _ |- _ =>
+    Hsuccess: AlgDom.dom_analysis_is_successful _ |- _ =>
      eapply (@TransCFG.pres_getEntryBlock (PhiPlacement pinfo)) 
        in Hentry; eauto;
      erewrite (@TransCFG.pres_has_no_predecessors (PhiPlacement pinfo)) 
