src3.0/Vellvm/Dominators/cfg.v
@@ -1,0 +1,215 @@
+Require Import List.
+Require Import ListSet.
+Require Import Coqlib.
+Require Import Metatheory.
+Require Import Maps.
+
+Require Import syntax.
+Require Import infrastructure.
+Require Import infrastructure_props.
+Import LLVMsyntax.
+Import LLVMinfra.
+
+Fixpoint successors_blocks (bs: blocks) : ATree.t ls :=
+match bs with
+| nil => ATree.empty ls
+| block_intro l0 _ _ tmn :: bs' =>
+    ATree.set l0 (successors_terminator tmn) (successors_blocks bs')
+end.
+
+Definition successors (f: fdef) : ATree.t ls :=
+let '(fdef_intro _ bs) := f in
+successors_blocks bs.
+
+Fixpoint bound_blocks (bs: blocks) : set atom :=
+match bs with
+| nil => empty_set _
+| block_intro l0 _ _ tmn :: bs' => l0::(bound_blocks bs')
+end.
+
+Definition bound_fdef (f: fdef) : set atom :=
+let '(fdef_intro _ bs) := f in
+bound_blocks bs.
+
+Require Import Dipaths.
+
+Definition vertexes_fdef (f:fdef) : V_set :=
+fun (v:Vertex) => let '(index a) := v in In a (bound_fdef f).
+
+Definition arcs_fdef (f:fdef) : A_set :=
+fun (arc:Arc) =>
+  let '(A_ends (index a2) (index a1)) := arc in
+  In a2 ((successors f)!!!a1).
+
+Lemma entry_in_vertexes : forall f l0 ps cs tmn
+  (Hentry : getEntryBlock f = Some (block_intro l0 ps cs tmn)),
+  vertexes_fdef f (index l0).
+Proof.
+  intros.
+  unfold vertexes_fdef. unfold bound_fdef. destruct f as [f b].
+  destruct b; simpl in *.
+    congruence.
+    inv Hentry. simpl. auto.
+Qed.
+
+Lemma in_successors_blocks__in_bound_blocks: forall (n : ATree.elt) (s : ls) 
+  (bs : blocks) (Hinscs : (successors_blocks bs) ! n = Some s),
+  In n (bound_blocks bs).
+Proof.
+  induction bs as [|[] bs]; simpl in *; intros.
+    rewrite ATree.gempty in Hinscs. congruence.
+
+    rewrite ATree.gsspec in Hinscs.
+    destruct_if; auto.
+Qed.
+
+Lemma in_parents__in_bound: forall bs n 
+  (Hparents: In n (XATree.parents_of_tree (successors_blocks bs))), 
+  In n (bound_blocks bs).
+Proof.
+  intros.
+  apply XATree.parents_of_tree__in_successors in Hparents.
+  destruct Hparents as [s Hinscs].
+  eapply in_successors_blocks__in_bound_blocks; eauto.
+Qed.
+
+Lemma successors__blockInFdefB : forall l0 a f,
+  In l0 (successors f) !!! a ->
+  exists ps0, exists cs0, exists tmn0,
+    blockInFdefB (block_intro a ps0 cs0 tmn0) f /\
+    In l0 (successors_terminator tmn0).
+Proof.
+  destruct f as [fh bs]. simpl.
+  unfold XATree.successors_list.
+  induction bs as [|a0 bs]; simpl; intro.
+    rewrite ATree.gempty in H. inv H.
+
+    destruct a0 as [l1 p c t].
+    destruct (id_dec l1 a); subst.
+      rewrite ATree.gss in H.
+      exists p. exists c. exists t.
+      split; auto.
+        eapply orb_true_iff. left. apply blockEqB_refl.
+
+      rewrite ATree.gso in H; auto.
+      apply IHbs in H; auto.
+      destruct H as [ps0 [cs0 [tmn0 [J1 J2]]]].
+      exists ps0. exists cs0. exists tmn0.
+      split; auto.
+        eapply orb_true_iff; eauto.
+Qed.
+
+Lemma successors_blocks__blockInFdefB : forall l0 a fh bs,
+  In l0 (successors_blocks bs) !!! a ->
+  exists ps0, exists cs0, exists tmn0,
+    blockInFdefB (block_intro a ps0 cs0 tmn0) (fdef_intro fh bs) /\
+    In l0 (successors_terminator tmn0).
+Proof.
+  intros.
+  apply successors__blockInFdefB; auto.
+Qed.
+
+Lemma successors_terminator__successors_blocks : forall
+  (bs : blocks)
+  (l0 : l)
+  (cs : phinodes)
+  (ps : cmds)
+  (tmn : terminator)
+  (l1 : l)
+  (HuniqF : uniqBlocks bs)
+  (HbInF : InBlocksB (block_intro l0 cs ps tmn) bs)
+  (Hin : In l1 (successors_terminator tmn)),
+  successors_terminator tmn = (successors_blocks bs) !!! l0.
+Proof.
+  intros.
+  induction bs.
+    inversion HbInF.
+
+    assert (J:=HuniqF).
+    simpl_env in J.
+    apply uniqBlocks_inv in J.
+    destruct J as [J1 J2].
+    simpl in *.
+    apply orb_prop in HbInF.
+    destruct a.
+    destruct HbInF as [HbInF | HbInF].
+      unfold blockEqB in HbInF.
+      apply sumbool2bool_true in HbInF. inv HbInF.
+      unfold XATree.successors_list.
+      rewrite ATree.gss. auto.
+
+      apply IHbs in J2; auto.
+      unfold XATree.successors_list in *.
+      destruct HuniqF as [J _].
+      inv J.
+      rewrite ATree.gso; auto.
+        clear - HbInF H1.
+        eapply InBlocksB__NotIn; eauto.
+Qed.
+
+Lemma successor_in_arcs : forall l0 cs ps tmn f l1
+  (HuniqF : uniqFdef f)
+  (HbInF : blockInFdefB (block_intro l0 cs ps tmn) f)
+  (Hin : In l1 (successors_terminator tmn)),
+  arcs_fdef f (A_ends (index l1) (index l0)).
+Proof.
+  intros.
+  unfold arcs_fdef.
+  destruct f as [fh bs]. apply uniqF__uniqBlocks in HuniqF.
+  simpl.
+  erewrite <- successors_terminator__successors_blocks; eauto.
+Qed.
+
+Lemma blockInFdefB_in_vertexes : forall l0 cs ps tmn f
+  (HbInF : blockInFdefB (block_intro l0 cs ps tmn) f),
+  vertexes_fdef f (index l0).
+Proof.
+  intros.
+  unfold vertexes_fdef, bound_fdef.
+  destruct f as [f b].
+  generalize dependent cs.
+  generalize dependent ps.
+  generalize dependent tmn.
+  generalize dependent l0.
+  induction b; simpl in *; intros.
+    congruence.
+
+    destruct a.
+    apply orb_prop in HbInF.
+    destruct HbInF as [HbInF | HbInF].
+      unfold blockEqB in HbInF.
+      apply sumbool2bool_true in HbInF. inv HbInF.
+      simpl. auto.
+
+      apply IHb in HbInF.
+      simpl. auto.
+Qed.
+
+Definition reachable (f:fdef) (l0:l) : Prop :=
+match getEntryBlock f with
+| Some (block_intro entry _ _ _) =>
+  let vertexes := vertexes_fdef f in
+  let arcs := arcs_fdef f in
+  exists vl: V_list, exists al: A_list,
+    D_walk vertexes arcs (index l0) (index entry) vl al
+| _ => false
+end.
+
+Definition domination (f:fdef) (l1 l2:l) : Prop :=
+match getEntryBlock f with
+| Some (block_intro entry _ _ _) =>
+  let vertexes := vertexes_fdef f in
+  let arcs := arcs_fdef f in
+  forall vl al,
+    D_walk vertexes arcs (index l2) (index entry) vl al ->
+    (In (index l1) vl \/ l1 = l2)
+| _ => False
+end.
+
+Definition strict_domination (f:fdef) (l1 l2:l) : Prop :=
+domination f l1 l2 /\ l1 <> l2.
+
+Definition imm_domination (f:fdef) (l1 l2:l) : Prop :=
+strict_domination f l1 l2 /\
+forall l0, strict_domination f l0 l2 -> domination f l0 l1.
+
