src3.0/Vellvm/Dominators/dom_decl.v
@@ -1,0 +1,318 @@
+Require Import List.
+Require Import ListSet.
+Require Import Coqlib.
+Require Import Metatheory.
+Require Import Maps.
+Require Import Lattice.
+Require Import Kildall.
+Require Import Iteration.
+Require Export cfg.
+Require Export reach.
+Require Import dom_type.
+Require Import Dipaths.
+
+Require Import syntax.
+Require Import infrastructure.
+Require Import infrastructure_props.
+Import LLVMsyntax.
+Import LLVMinfra.
+
+Module DecDom.
+
+Lemma dom_tran: forall (f:fdef) (l1 l2 l3:l),
+  domination f l1 l2 -> domination f l2 l3 -> domination f l1 l3.
+Proof.
+  unfold domination.
+  intros.
+  destruct (getEntryBlock f); tinv H.
+  destruct b.
+  intros vl al Hw.
+  destruct (id_dec l1 l3); auto.
+  left.
+  assert (Hw':=Hw).
+  apply H0 in Hw'.
+  destruct Hw' as [Hw' | Hw']; subst.
+    apply DW_extract with (x:=index l2)(eq_a_dec:=eq_atom_dec) in Hw; 
+      simpl; auto.
+    destruct Hw as [al' Hw].
+    assert (Hw'':=Hw).
+    apply H in Hw''.
+    destruct Hw'' as [Hw'' | Hw'']; subst; auto.
+    destruct (id_dec l1 l2); subst; auto.
+    apply V_extract_spec in Hw''; try congruence.
+    simpl in Hw''. destruct Hw'' as [Hw'' | Hw'']; congruence.
+
+    assert (Hw'':=Hw).
+    apply H in Hw''.
+    destruct Hw'' as [Hw'' | Hw'']; subst; congruence.
+Qed.
+
+Section dom_acyclic_tran.
+
+Variable f:fdef.
+
+Hypothesis getEntryBlock_inv : forall
+  (l3 : l)
+  (l' : l)
+  (ps : phinodes)
+  (cs : cmds)
+  (tmn : terminator)
+  (HBinF : blockInFdefB (block_intro l3 ps cs tmn) f = true)
+  (Hsucc : In l' (successors_terminator tmn)) a ps0 cs0 tmn0
+  (H : getEntryBlock f = Some (block_intro a ps0 cs0 tmn0)),
+  l' <> a.
+
+Lemma dom_acyclic: forall (l1 l2:l)
+  (H: reachable f l2) (H0: strict_domination f l1 l2),
+  ~ domination f l2 l1.
+Proof.
+  unfold reachable, strict_domination, domination.
+  intros. 
+  remember (getEntryBlock f) as R.
+  destruct R; auto. 
+  destruct b as [l0 ? ? ?].
+  destruct H as [vl [al Hw]].
+  apply DWalk_to_dpath in Hw; auto.
+  destruct Hw as [vl0 [al0 Hp]].
+  assert (Hw:=Hp).
+  apply D_path_isa_walk in Hw.
+  destruct H0 as [J1 J2].
+  assert (Hw':=Hw).
+  apply J1 in Hw'.
+  destruct Hw' as [Hw' | Hw']; subst; try congruence.
+  intros J.
+  apply DW_extract with (x:=index l1)(eq_a_dec:=eq_atom_dec) in Hw; 
+    simpl; auto.
+  destruct Hw as [al' Hw].
+  assert (Hw'':=Hw).
+  apply J in Hw''.
+  destruct Hw'' as [Hw'' | Hw'']; subst; auto.
+  apply V_extract_spec' in Hw''; try congruence.
+  inv Hp.
+    inv Hw'.
+
+    simpl in Hw''.
+    destruct Hw'' as [Hw'' | Hw'']; subst; try congruence.
+    apply H4 in Hw''. inv Hw''.
+    destruct y as [a0].
+    assert (exists ps0, exists cs0, exists tmn0,
+      blockInFdefB (block_intro a0 ps0 cs0 tmn0) f /\
+      In l0 (successors_terminator tmn0)) as J'.
+      eapply successors__blockInFdefB; eauto.
+    destruct J' as [ps0 [cs0 [tmn0 [HBinF' Hinsucc]]]].
+    symmetry in HeqR. 
+    eapply getEntryBlock_inv in Hinsucc; eauto.
+Qed.
+
+Lemma sdom_tran1: forall (l1 l2 l3:l) (Hreach: reachable f l2),
+  strict_domination f l1 l2 -> domination f l2 l3 -> strict_domination f l1 l3.
+Proof.
+  intros.
+  destruct (id_dec l1 l3); subst.
+    eapply dom_acyclic in H; eauto.
+    contradict H; auto.
+
+    destruct H.
+    split; eauto using dom_tran.
+Qed.
+
+Lemma sdom_tran2: forall (l1 l2 l3:l) (Hreach: reachable f l3),
+  domination f l1 l2 -> strict_domination f l2 l3 -> strict_domination f l1 l3.
+Proof.
+  intros.
+  destruct (id_dec l1 l3); subst.
+    eapply dom_acyclic in H0; eauto.
+    contradict H0; auto.
+
+    destruct H0.
+    split; eauto using dom_tran.
+Qed.
+
+Lemma sdom_tran: forall (l1 l2 l3:l) (Hreach: reachable f l2),
+  strict_domination f l1 l2 -> strict_domination f l2 l3 ->
+  strict_domination f l1 l3.
+Proof.
+  intros. destruct H0. eapply sdom_tran1; eauto.
+Qed.
+
+End dom_acyclic_tran.
+
+Lemma sdom_reachable : forall f l1 l2,
+  reachable f l2 -> strict_domination f l1 l2 -> reachable f l1.
+Proof.
+  unfold reachable, strict_domination, domination.
+  intros.
+  destruct H0 as [J1 J2].
+  destruct (getEntryBlock f); try congruence.
+  destruct b.
+  destruct H as [vl [al H]].
+  assert (H':=H).
+  apply J1 in H'.
+  assert (In (index l1) vl) as Hin.
+    destruct H' as [H' | H']; subst; try congruence.
+  apply DW_extract with (x:=index l1)(eq_a_dec:=eq_atom_dec) in H; 
+    simpl; auto.
+  destruct H as [al' H].
+  exists (V_extract eq_atom_dec (index l1) (index l2 :: vl)). exists al'.
+  auto.
+Qed.
+
+Lemma dom_reachable : forall f l1 l2,
+  reachable f l2 -> domination f l1 l2 -> reachable f l1.
+Proof.
+  intros.
+  destruct (id_dec l1 l2); subst; auto.
+  eapply sdom_reachable; eauto. split; auto.
+Qed.
+
+Lemma sdom_dec : forall f l1 l2,
+  strict_domination f l1 l2 \/ ~ strict_domination f l1 l2.
+Proof. intros. tauto. Qed. (* classic logic *)
+
+Lemma everything_dominates_unreachable_blocks :
+  forall f l1 l2 (Hreach: ~ reachable f l2)
+  (Hentry: getEntryBlock f <> None),
+  domination f l1 l2.
+Proof.
+  unfold reachable, domination.
+  intros.
+  destruct (getEntryBlock f); try congruence.
+  destruct b.
+  intros.
+  contradict Hreach. eauto.
+Qed.
+
+Lemma tauto_helper : forall A B:Prop,
+  A -> ~ (B /\ A) -> ~ B.
+Proof. tauto. Qed.
+
+Import Classical_Pred_Type.
+
+Lemma sdom_ordered : forall f l1 l2 l3
+  (Hneq: l1 <> l2) (Hreach: reachable f l3)
+  (Hsdom: strict_domination f l1 l3)
+  (Hsdom': strict_domination f l2 l3),
+  strict_domination f l1 l2 \/ strict_domination f l2 l1.
+Proof.
+  intros.
+  destruct (sdom_dec f l1 l2); auto.
+  destruct (sdom_dec f l2 l1); auto.
+  contradict Hsdom'. intro Hsdom'.
+  unfold strict_domination in *.
+  destruct Hsdom as [Hdom Hneq1].
+  destruct Hsdom' as [Hdom' Hneq2].
+  unfold domination, reachable in *.
+  destruct (getEntryBlock f); auto.
+  destruct b as [l0 ? ? ?].
+  destruct Hreach as [vl [al Hreach]].
+  assert (Hw:=Hreach).
+  apply Hdom in Hw.
+  destruct Hw as [Hin | Heq]; try congruence.
+  assert (Hw:=Hreach).
+  apply Hdom' in Hw.
+  destruct Hw as [Hin' | Heq]; try congruence.
+
+  (* on Hw, we need to figuire the closest one to l3 in l1 and l2,
+     suppose l1 is, then we split hw at l1, so l2 cannot be in the part
+     from l3 to l1.
+  *)
+  assert (Hw:=Hreach).
+  assert (vl <> V_nil) as Hnqnil.
+    destruct vl; auto.
+      intro J. inv J.
+  apply DW_cut with (x:=index l1) (w:=index l2) in Hw; try congruence;
+    simpl; auto.
+  destruct Hw as [al1 [al2 [vl1 [vl2
+    [[J1 [J2 [J3 [J4 J5]]]]|[J1 [J2 [J3 [J4 J5]]]]]]]]]; subst.
+  Case "1".
+  assert (exists vl:V_list, exists al:A_list,
+    D_walk (vertexes_fdef f) (arcs_fdef f) (index l1) (index l0) vl al /\
+    ~ In (index l2) vl) as J.
+    clear - Hneq H0.
+    apply tauto_helper in H0; auto.
+    apply not_all_ex_not in H0. (* can we remove the classic lemma? *)
+    destruct H0 as [vl H0].
+    apply not_all_ex_not in H0.
+    destruct H0 as [al H0].
+    exists vl. exists al.
+    tauto.
+  destruct J as [vl1' [al1' [J1' J2']]].
+
+  assert ((D_walk (vertexes_fdef f) (arcs_fdef f) (index l3) (index l0)
+    (vl1++vl1') (al1++al1') * ~ In (index l2) (vl1++vl1'))%type) as J.
+    split.
+      eapply DWalk_append; eauto.
+
+      clear - J2' J5.
+      intro J. apply in_app_or in J.
+      simpl in *.
+      destruct J as [J | J]; auto.
+  destruct J as [J3 J4].
+  apply Hdom' in J3.
+  destruct J3 as [Hin'' | Heq]; try congruence.
+
+  Case "2".
+  assert (exists vl:V_list, exists al:A_list,
+    D_walk (vertexes_fdef f) (arcs_fdef f) (index l2) (index l0) vl al /\
+    ~ In (index l1) vl) as J.
+    clear - Hneq H.
+    apply tauto_helper in H; auto.
+    apply not_all_ex_not in H.
+    destruct H as [vl H].
+    apply not_all_ex_not in H.
+    destruct H as [al H].
+    exists vl. exists al.
+    tauto.
+  destruct J as [vl2' [al2' [J1' J2']]].
+
+  assert ((D_walk (vertexes_fdef f) (arcs_fdef f) (index l3) (index l0)
+    (vl1++vl2') (al1++al2') * ~ In (index l1) (vl1++vl2'))%type) as J.
+    split.
+      eapply DWalk_append; eauto.
+
+      clear - J2' J5.
+      intro J. apply in_app_or in J.
+      simpl in *.
+      destruct J as [J | J]; auto.
+  destruct J as [J3 J4].
+  apply Hdom in J3.
+  destruct J3 as [Hin'' | Heq]; try congruence.
+Qed.
+
+Lemma non_sdom__inv: forall f l1 l2 be (Hentry: getEntryBlock f = Some be)
+  (Hnsdom: ~ strict_domination f l1 l2),
+  l1 = l2 \/ 
+  exists vl, exists al, D_walk (vertexes_fdef f) (arcs_fdef f) 
+    (index l2) (index (getBlockLabel be)) vl al /\
+    ~ In (index l1) vl.
+Proof.
+  intros.
+  destruct (l_dec l1 l2); subst; auto.
+  right.
+  assert (
+   (exists p : (V_list * A_list),
+      D_walk (vertexes_fdef f) (arcs_fdef f) (index l2)
+        (index (getBlockLabel be)) (fst p) (snd p) /\ 
+        ~ In (index l1) (fst p)) ->
+   exists vl : V_list,
+     exists al : A_list,
+       D_walk (vertexes_fdef f) (arcs_fdef f) (index l2)
+         (index (getBlockLabel be)) vl al /\ ~ In (index l1) vl
+  ) as G.
+    intros [[vl al] J]. eauto.
+  apply G. clear G.
+  apply Classical_Pred_Type.not_all_not_ex.
+  intro J.
+  apply Hnsdom.
+  unfold strict_domination, domination.
+  fill_ctxhole.
+  split; auto.
+    destruct be.
+    intros vl al Hwalk.
+    left.
+    destruct (In_dec (V_eq_dec eq_atom_dec) (index l1) vl); auto.
+      assert (G:=J (vl,al)). clear J.
+      contradict G. auto.
+Qed.
+
+End DecDom.
