src3.0/Vellvm/Dominators/dom_set.v
@@ -1,0 +1,1236 @@
+Require Import List.
+Require Import ListSet.
+Require Import Coqlib.
+Require Import Metatheory.
+Require Import Maps.
+Require Import Lattice.
+Require Import Kildall.
+Require Import Iteration.
+Require Export cfg.
+Require Export reach.
+Require Export dom_decl.
+Require Import dom_type.
+Require Import Dipaths.
+
+Require Import syntax.
+Require Import infrastructure.
+Require Import infrastructure_props.
+Import LLVMsyntax.
+Import LLVMinfra.
+
+Module AlgDom : ALGDOM.
+
+Definition transfer (lbl: l) (before: Dominators.t) :=
+  Dominators.add before lbl.
+
+(** The static analysis itself is then an instantiation of Kildall's
+  generic solver for forward dataflow inequations. [analyze f]
+  returns a mapping from program points to mappings of pseudo-registers
+  to approximations.  It can fail to reach a fixpoint in a reasonable
+  number of iterations, in which case [None] is returned. *)
+
+Module DomDS := Dataflow_Solver_Var_Top(AtomNodeSet).
+
+Definition dom_analyze (f: fdef) : AMap.t Dominators.t :=
+  let '(fdef_intro _ bs) := f in
+  let top := Dominators.top in
+  match getEntryBlock f with
+  | Some (block_intro le _ _ _) =>
+      match DomDS.fixpoint (successors_blocks bs) transfer
+        ((le, top) :: nil) with
+      | None => AMap.init top
+      | Some res => res
+      end
+  | None => AMap.init top
+  end.
+
+Definition dom_analysis_is_successful (f: fdef) : Prop :=
+  let '(fdef_intro _ bs) := f in
+  let top := Dominators.top in
+  match getEntryBlock f with
+  | Some (block_intro le _ _ _) =>
+      match DomDS.fixpoint (successors_blocks bs) transfer
+        ((le, top) :: nil) with
+      | None => False
+      | Some res => True
+      end
+  | None => False
+  end.
+
+Definition bound_dom bd (res: Dominators.t) : set atom :=
+match res with
+| Some dts2 => dts2
+| None => bd
+end.
+
+Definition dom_query f : atom -> set atom :=
+let dt := dom_analyze f in
+let b := bound_fdef f in
+fun l0 => bound_dom b (dt !! l0).
+
+Import AtomSet.
+
+Lemma dom_entrypoint : forall f l0 ps cs tmn
+  (Hentry : getEntryBlock f = Some (block_intro l0 ps cs tmn)),
+  dom_query f l0 = nil.
+Proof.
+  intros.
+  unfold dom_query, dom_analyze.
+  destruct f as [f b].
+  rewrite Hentry.
+  remember (DomDS.fixpoint (successors_blocks b)
+                transfer ((l0, Dominators.top) :: nil)) as R1.
+  destruct R1; subst.
+  SCase "analysis is done".
+    symmetry in HeqR1.
+    apply DomDS.fixpoint_entry with (n:=l0)(v:=Some nil) in HeqR1; simpl; eauto.
+    unfold DomDS.L.ge, DomDS.L.sub in HeqR1.
+    destruct (t !! l0); try tauto.
+      apply incl_empty_inv in HeqR1; subst; auto.
+
+  SCase "analysis fails".
+    rewrite AMap.gi. auto.
+Qed.
+
+Module EntryDomsOthers. Section EntryDomsOthers.
+
+Variable bs : blocks.
+Definition predecessors := XATree.make_predecessors (successors_blocks bs).
+Definition transf := transfer.
+Definition top := Dominators.top.
+Definition bot := Dominators.bot.
+Variable entry: l.
+Variable entrypoints: list (atom * DomDS.L.t).
+
+Hypothesis wf_entrypoints:
+  predecessors!!!entry = nil /\
+  match bs with
+  | block_intro l0 _ _ _ :: _ => l0 = entry
+  | _ => False
+  end /\
+  exists v, [(entry, v)] = entrypoints /\ Dominators.eq v top.
+
+Lemma dom_entry_start_state_in:
+  forall n v,
+  In (n, v) entrypoints ->
+  Dominators.eq (DomDS.start_state_in entrypoints)!!n v.
+Proof.
+  destruct wf_entrypoints as [_ [_ J]]. clear wf_entrypoints.
+  destruct J as [v [Heq J]]; subst. simpl.
+  intros.
+  destruct H as [H | H]; inv H.
+  rewrite AMap.gss. rewrite AMap.gi.
+  apply Dominators.eq_trans with (y:=DomDS.L.lub v0 bot).
+    apply Dominators.lub_commut.
+    apply Dominators.lub_preserves_ge.
+    apply Dominators.ge_compat with (x:=top)(y:=bot).
+      apply Dominators.eq_sym; auto.
+      apply Dominators.eq_refl.
+      apply Dominators.ge_bot.
+Qed.
+
+Lemma dom_nonentry_start_state_in:
+  forall n,
+  n <> entry ->
+  Dominators.eq (DomDS.start_state_in entrypoints)!!n bot.
+Proof.
+  destruct wf_entrypoints as [_ [_ J]]. clear wf_entrypoints.
+  destruct J as [v [Heq J]]; subst. simpl.
+  intros.
+  rewrite AMap.gi. rewrite AMap.gso; auto. rewrite AMap.gi.
+  apply Dominators.eq_refl.
+Qed.
+
+Lemma transf_mono: forall p x y,
+  Dominators.ge x y -> Dominators.ge (transf p x) (transf p y).
+Proof.
+  unfold transf, transfer. intros.
+  apply Dominators.add_mono; auto.
+Qed.
+
+Definition lub_of_preds (res: AMap.t DomDS.L.t) (n:atom) : DomDS.L.t :=
+  Dominators.lubs (List.map (fun p => transf p res!!p)
+    (predecessors!!!n)).
+
+Definition entry_doms_others (res: AMap.t DomDS.L.t) : Prop :=
+  forall l0, l0 <> entry -> Dominators.member entry res!!l0.
+
+Lemma start_entry_doms_others:
+  entry_doms_others
+    (DomDS.st_in (DomDS.start_state (successors_blocks bs) entrypoints)).
+Proof.
+  intros l0 Hneq.
+  apply dom_nonentry_start_state_in in Hneq.
+  unfold DomDS.start_state. simpl.
+  apply Dominators.member_eq with (x2:=bot); auto.
+  destruct wf_entrypoints as [_ [J _]]. unfold bot.
+  destruct bs; tinv J.
+  destruct b; subst. simpl. auto.
+Qed.
+
+(** We show that the start state satisfies the invariant, and that
+  the [step] function preserves it. *)
+
+Lemma propagate_succ_entry_doms_others: forall st n out,
+  Dominators.member entry out ->
+  entry_doms_others st.(DomDS.st_in) ->
+  entry_doms_others (DomDS.propagate_succ st out n).(DomDS.st_in).
+Proof.
+  unfold entry_doms_others.
+  intros.
+  destruct (@DomDS.propagate_succ_spec st out n) as [J1 J2].
+  apply H0 in H1.
+  destruct (eq_atom_dec n l0); subst.
+    apply Dominators.member_eq with (a:=entry) in J1; auto.
+    apply Dominators.member_lub; auto.
+
+    rewrite J2; auto.
+Qed.
+
+Lemma propagate_succ_list_entry_doms_others:
+  forall scs st out,
+  Dominators.member entry out ->
+  entry_doms_others st.(DomDS.st_in) ->
+  entry_doms_others (DomDS.propagate_succ_list st out scs).(DomDS.st_in).
+Proof.
+  induction scs; simpl; intros; auto.
+    apply IHscs; auto.
+    apply propagate_succ_entry_doms_others; auto.
+Qed.
+
+Lemma step_entry_doms_others:
+  forall st n rem,
+  AtomNodeSet.pick st.(DomDS.st_wrk) = Some(n, rem) ->
+  entry_doms_others st.(DomDS.st_in) ->
+  entry_doms_others (DomDS.propagate_succ_list
+                                  (DomDS.mkstate st.(DomDS.st_in) rem)
+                                  (transf n st.(DomDS.st_in)!!n)
+                                  ((successors_blocks bs)!!!n)).(DomDS.st_in).
+Proof.
+  intros st n rem WKL GOOD.
+  destruct st. simpl.
+  apply propagate_succ_list_entry_doms_others; auto.
+    simpl in *.
+    unfold transf, transfer.
+    destruct (eq_atom_dec n entry); subst.
+      apply Dominators.add_member1.
+      destruct wf_entrypoints as [_ [J _]].
+      destruct bs; tinv J.
+      destruct b; subst. simpl. auto.
+
+      apply GOOD in n0.
+      apply Dominators.add_member2; auto.
+Qed.
+
+Theorem dom_entry_doms_others: forall res,
+  DomDS.fixpoint (successors_blocks bs) transf entrypoints = Some res ->
+  entry_doms_others res.
+Proof.
+  unfold DomDS.fixpoint. intros res PI. pattern res.
+  eapply (PrimIter.iterate_prop _ _ (DomDS.step _ _)
+    (fun st => entry_doms_others st.(DomDS.st_in))); eauto.
+  intros st GOOD. unfold DomDS.step.
+  caseEq (AtomNodeSet.pick st.(DomDS.st_wrk)); auto.
+  intros [n rem] PICK.
+  apply step_entry_doms_others; auto.
+    apply start_entry_doms_others.
+Qed.
+
+Lemma dom_solution_ge: forall res,
+  DomDS.fixpoint (successors_blocks bs) transf entrypoints = Some res ->
+  forall n,
+  Dominators.ge res!!n (lub_of_preds res n).
+Proof.
+  intros.
+  apply Dominators.lubs_spec3.
+  intros.
+  apply in_map_iff in H0.
+  destruct H0 as [x [J1 J2]]; subst.
+  eapply DomDS.fixpoint_solution; eauto.
+  apply XATree.make_predecessors_correct'; auto.
+Qed.
+
+End EntryDomsOthers. End EntryDomsOthers.
+
+Definition wf_entrypoints f: Prop :=
+  match getEntryBlock f with
+  | Some (block_intro l0 _ _ _) => 
+      (XATree.make_predecessors (successors f))!!!l0 = nil
+  | _ => False
+  end.
+
+Section entry_doms_others.
+
+Variable f:fdef.
+
+Hypothesis wf_entrypoints: wf_entrypoints f.
+
+Lemma entry_doms_others: forall
+  entry
+  (Hex: dom_analysis_is_successful f)
+  (H: getEntryLabel f = Some entry),
+  (forall b (H0: b <> entry /\ reachable f b),
+     ListSet.set_In entry (AlgDom.dom_query f b)).
+Proof.
+  intros.
+  destruct H0 as [J1 J2].
+  unfold dom_query, dom_analyze.
+  unfold dom_analysis_is_successful in Hex.
+  destruct f as [fh b0].
+  remember (getEntryBlock (fdef_intro fh b0)) as R.
+  destruct R as [[l1 p c t]|]; try tauto.
+  destruct b0 as [|b0 b2]; inv HeqR.
+  inv H.
+  remember (
+      DomDS.fixpoint 
+           (successors_blocks (block_intro entry p c t :: b2))
+           transfer
+           ((entry, Dominators.top) :: nil)) as R.
+  destruct R; try tauto.
+  symmetry in HeqR.
+  eapply EntryDomsOthers.dom_entry_doms_others with (entry:=entry) in HeqR; 
+    eauto.
+  Case "1".
+    unfold EntryDomsOthers.entry_doms_others in HeqR.
+    apply HeqR in J1.
+    unfold Dominators.member in J1.
+    destruct (t0 !! b); simpl; auto.
+
+  Case "2".
+    split; auto.
+    split; auto.
+      exists Dominators.top.
+      simpl.
+      split; auto.
+        split; intros x Hin; auto.
+Qed.
+
+End entry_doms_others.
+
+Module DomsInParents. Section DomsInParents.
+
+Variable succs : ATree.t (list l).
+Definition transf := transfer.
+Definition top := Dominators.top.
+Definition bot := Dominators.bot.
+Variable entry: l.
+Definition entrypoints : list (atom * DomDS.L.t) := (entry, Dominators.top)::nil.
+
+Definition wf_dom (res: DomDS.L.t) : Prop :=
+  match res with
+  | Some ns0 => incl ns0 (XATree.parents_of_tree succs)
+  | None => True
+  end.
+
+Definition wf_doms (res: AMap.t DomDS.L.t) : Prop := 
+  forall l0, wf_dom (res !! l0).
+
+Lemma start_wf_doms:
+  wf_doms (DomDS.st_in (DomDS.start_state succs entrypoints)).
+Proof.
+  simpl. intros l0.
+  rewrite AMap.gsspec.
+  rewrite AMap.gi. simpl. 
+  destruct_if; simpl.
+    intros x Hinx. inv Hinx.
+    rewrite AMap.gi. simpl. auto.
+Qed.
+
+(** We show that the start state satisfies the invariant, and that
+  the [step] function preserves it. *)
+
+Lemma wf_dom_eq: forall dt1 dt2 (Heq: DomDS.L.eq dt1 dt2) (Hwf: wf_dom dt2),
+  wf_dom dt1.
+Proof.
+  unfold wf_dom.
+  intros.
+  destruct dt1; destruct dt2; tinv Heq; auto.
+    elim Heq. intros. eauto with datatypes v62.
+Qed.
+
+Lemma propagate_succ_wf_doms: forall st n out,
+  wf_dom out ->
+  wf_doms st.(DomDS.st_in) ->
+  wf_doms (DomDS.propagate_succ st out n).(DomDS.st_in).
+Proof.
+  unfold wf_doms.
+  intros.
+  destruct (@DomDS.propagate_succ_spec st out n) as [J1 J2].
+  destruct (eq_atom_dec n l0); subst.
+    apply wf_dom_eq in J1; auto.
+    assert (J:=H0 l0).
+    clear - J H.
+    unfold wf_dom in *.
+    destruct out, (DomDS.st_in st) !! l0; simpl; auto.
+      apply incl_inter_left; auto.
+
+    rewrite J2; auto.
+Qed.
+
+Lemma propagate_succ_list_wf_doms:
+  forall scs st out (Hsc: scs <> nil -> wf_dom out),
+  wf_doms st.(DomDS.st_in) ->
+  wf_doms (DomDS.propagate_succ_list st out scs).(DomDS.st_in).
+Proof.
+  induction scs; simpl; intros; auto.
+    apply IHscs; auto.
+      intro J. apply Hsc. congruence.
+      apply propagate_succ_wf_doms; auto.
+        apply Hsc. congruence.
+Qed.
+
+Lemma step_wf_doms:
+  forall st n rem,
+  AtomNodeSet.pick st.(DomDS.st_wrk) = Some(n, rem) ->
+  wf_doms st.(DomDS.st_in) ->
+  wf_doms (DomDS.propagate_succ_list
+             (DomDS.mkstate st.(DomDS.st_in) rem)
+             (transf n st.(DomDS.st_in)!!n)
+             (succs!!!n)).(DomDS.st_in).
+Proof.
+  intros st n rem WKL GOOD.
+  destruct st. simpl.
+  apply propagate_succ_list_wf_doms; auto.
+    intro Hnnil.
+    assert (J:=GOOD n). simpl in J.
+    unfold wf_dom. unfold wf_dom in J.    
+    destruct (st_in !! n); simpl; auto.
+    intros x Hin.
+    destruct_in Hin; auto.
+      apply XATree.nonleaf_is_parent; auto.
+Qed.
+
+Theorem fixpoint_wf: forall res,
+  DomDS.fixpoint succs transf entrypoints = Some res ->
+  wf_doms res.
+Proof.
+  unfold DomDS.fixpoint. intros res PI. pattern res.
+  eapply (PrimIter.iterate_prop _ _ (DomDS.step _ _)
+    (fun st => wf_doms st.(DomDS.st_in))); eauto.
+    intros st GOOD. unfold DomDS.step.
+    caseEq (AtomNodeSet.pick st.(DomDS.st_wrk)); auto.
+    intros [n rem] PICK.
+    apply step_wf_doms; auto.
+
+    apply start_wf_doms.
+Qed.
+
+End DomsInParents. End DomsInParents.
+
+Lemma dom_in_bound: forall successors le t
+  (Hfix: DomDS.fixpoint successors transfer
+            ((le, Dominators.top) :: nil) = Some t),
+  forall l0 ns0 (Hget: t !! l0 = Some ns0) n (Hin: In n ns0),
+    In n (XATree.parents_of_tree successors).
+Proof.
+  intros.
+  apply DomsInParents.fixpoint_wf in Hfix; auto.
+  assert (J:=Hfix l0).
+  unfold DomsInParents.wf_dom in J.
+  rewrite Hget in J. auto.
+Qed.
+
+Lemma dom_in_bound_blocks: forall bs le t
+  (Hfix: DomDS.fixpoint (successors_blocks bs) transfer
+            ((le, Dominators.top) :: nil) = Some t),
+  forall l0 ns0 (Hget: t !! l0 = Some ns0), incl ns0 (bound_blocks bs).
+Proof.
+  intros.
+  intros x Hinx.
+  apply in_parents__in_bound.
+  eapply dom_in_bound; eauto.
+Qed.
+
+Lemma dom_query_in_bound: forall fh bs l5, 
+  incl (dom_query (fdef_intro fh bs) l5) (bound_blocks bs).
+Proof.
+  intros.
+  unfold dom_query, dom_analyze.
+  destruct (getEntryBlock (fdef_intro fh bs)) as [[]|]; simpl. 
+    remember (DomDS.fixpoint (successors_blocks bs) transfer
+                ((l0, Dominators.top) :: nil)) as R.
+    destruct R.
+      symmetry in HeqR.
+      remember (t !! l5) as R.
+      destruct R; simpl; auto with datatypes v62.
+        eapply dom_in_bound_blocks; eauto.
+
+      rewrite AMap.gi. simpl. intros x Hin. inv Hin.
+    rewrite AMap.gi. simpl. intros x Hin. inv Hin.
+Qed.
+
+Lemma in_bound_dom__in_bound_fdef: forall l' f l1
+  (Hin: In l' (dom_query f l1)),
+  In l' (bound_fdef f).
+Proof.
+  intros. destruct f. eapply dom_query_in_bound; eauto.
+Qed.
+
+Lemma dom_successors : forall
+  (l3 : l) (l' : l) f
+  (contents3 contents': ListSet.set atom)
+  (Hinscs : In l' (successors f) !!! l3)
+  (Heqdefs3 : contents3 = dom_query f l3)
+  (Heqdefs' : contents' = dom_query f l'),
+  incl contents' (l3 :: contents3).
+Proof.
+  intros. 
+  unfold dom_query, dom_analyze in *.
+  remember (getEntryBlock f) as R.
+  destruct f as [fh bs].
+  destruct R as [[le ? ? ?]|].
+  Case "entry is good".
+    remember (DomDS.fixpoint (successors_blocks bs)
+                transfer ((le, Dominators.top) :: nil)) as R1.
+    destruct R1; subst.
+    SCase "analysis is done".
+      symmetry in HeqR1.
+      assert (Hinbd: forall l0 ns0 (Hget: t !! l0 = Some ns0), 
+                     incl ns0 (bound_blocks bs)).
+        eapply dom_in_bound_blocks; eauto.
+      apply DomDS.fixpoint_solution with (s:=l')(n:=l3) in HeqR1; eauto.
+      unfold transfer, DomDS.L.ge, DomDS.L.sub, Dominators.add in HeqR1.
+      remember (t !! l') as R2.
+      remember (t !! l3) as R3.
+      destruct R2 as [els2|]; destruct R3 as [els3|]; 
+        simpl; try solve [auto with datatypes v62 | tauto].
+        symmetry in HeqR2.
+        apply Hinbd in HeqR2. auto with datatypes v62.
+
+    SCase "analysis fails".
+      repeat rewrite AMap.gi. simpl. auto with datatypes v62.
+
+  Case "entry is wrong".
+    subst. repeat rewrite AMap.gi. simpl. auto with datatypes v62.
+Qed.
+
+Module DomComplete. Section DomComplete.
+
+Variable fh : fheader.
+Variable bs : blocks.
+Definition predecessors := XATree.make_predecessors (successors_blocks bs).
+Definition transf := transfer.
+Definition top := Dominators.top.
+Definition bot := Dominators.bot.
+Variable entry: l.
+Variable entrypoints: list (atom * DomDS.L.t).
+
+Hypothesis wf_entrypoints:
+  predecessors!!!entry = nil /\
+  match bs with
+  | block_intro l0 _ _ _ :: _ => l0 = entry
+  | _ => False
+  end /\
+  exists v, [(entry, v)] = entrypoints /\ Dominators.eq v top.
+
+Definition non_sdomination (l1 l2:l) : Prop :=
+  let vertexes := vertexes_fdef (fdef_intro fh bs) in
+  let arcs := arcs_fdef (fdef_intro fh bs) in
+  exists vl, exists al,
+    D_walk vertexes arcs (index l2) (index entry) vl al /\
+    ~ In (index l1) vl.
+
+Definition non_sdomination_prop (res: AMap.t DomDS.L.t) : Prop :=
+  forall l1 l2,
+    vertexes_fdef (fdef_intro fh bs) (index l1) ->
+    ~ Dominators.member l1 res!!l2 ->
+    non_sdomination l1 l2.
+
+Lemma start_non_sdomination:
+  non_sdomination_prop
+    (DomDS.st_in (DomDS.start_state (successors_blocks bs) entrypoints)).
+Proof.
+  intros l1 l2 Hin Hnotin.
+  destruct (eq_atom_dec l2 entry); try subst l2.
+    unfold non_sdomination.
+    exists V_nil. exists A_nil.
+    split.
+      constructor.
+      destruct wf_entrypoints as [_ [J _]].
+      destruct bs; tinv J.
+      destruct b; subst.
+      eapply entry_in_vertexes; simpl; eauto.
+
+      intro J. inv J.
+
+    eapply EntryDomsOthers.dom_nonentry_start_state_in in n; eauto.
+    contradict Hnotin.
+    unfold DomDS.start_state. simpl.
+    apply Dominators.member_eq with (x2:=bot); simpl; auto.
+Qed.
+
+Lemma non_sdomination_refl : forall l1,
+  l1 <> entry ->
+  reachable (fdef_intro fh bs) l1 ->
+  non_sdomination l1 l1.
+Proof.
+  unfold reachable, non_sdomination.
+  intros.
+  destruct bs; simpl in *.
+    inv H0.
+    destruct b; simpl in *.
+    destruct H0 as [vl [al H0]].
+    apply DWalk_to_dpath in H0; auto.
+    destruct H0 as [vl0 [al0 Hp]].
+    exists vl0. exists al0.
+    destruct wf_entrypoints as [_ [Heq _]]; subst.
+    split.
+      apply D_path_isa_walk; auto.
+      eapply DP_endx_ninV; eauto. congruence.
+Qed.
+
+Hypothesis branches_in_vertexes: forall p ps0 cs0 tmn0 l2
+  (J3 : blockInFdefB (block_intro p ps0 cs0 tmn0) (fdef_intro fh bs))
+  (J4 : In l2 (successors_terminator tmn0)),
+  vertexes_fdef (fdef_intro fh bs) (index l2).
+(*
+          eapply wf_fdef__blockInFdefB__wf_block in J3; eauto.
+          inv J3. inv HwfF.
+          match goal with
+          | H12: wf_insn _ _ _ _ _ |- _ =>
+            eapply wf_tmn__in_successors in H12; eauto;
+            destruct H12 as [cs1 [ps1 [tmn1 H12]]]
+          end.
+          eapply blockInFdefB_in_vertexes; eauto.
+*)
+
+Hypothesis UniqF: uniqFdef (fdef_intro fh bs).
+
+Lemma propagate_succ_non_sdomination: forall st p n out
+  (Hinpds: In p predecessors!!!n)
+  (Hout: Dominators.ge (transf p st.(DomDS.st_in)!!p) out)
+  (Hdom: non_sdomination_prop st.(DomDS.st_in)),
+  non_sdomination_prop (DomDS.propagate_succ st out n).(DomDS.st_in).
+Proof.
+  unfold non_sdomination_prop. intros.
+  destruct (@DomDS.propagate_succ_spec st out n) as [J1 J2].
+  destruct (eq_atom_dec n l2) as [Heq | Hneq]; subst.
+  Case "n=l2".
+    destruct (Dominators.member_dec l1 (DomDS.st_in st) !! l2)
+      as [Hin12 | Hnotin12]; auto.
+    assert (~ Dominators.member l1
+      (DomDS.L.lub (DomDS.st_in st) !! l2 out)) as Hnotlub12.
+      intro J. apply H0.
+      eapply Dominators.member_eq; eauto.
+    clear J1 J2.
+    destruct (Dominators.member_dec l1 out) as [Hinout | Hnotout]; auto.
+    SCase "l1 in out".
+      contradict Hnotlub12. apply Dominators.lub_intro; auto.
+    SCase "l1 notin out".
+      assert (~ Dominators.member l1 (transf p (DomDS.st_in st) !! p))
+        as Hnotintransf.
+        intro J. apply Hnotout.
+        eapply Dominators.ge_elim in Hout; eauto.
+      unfold transf, transfer in Hnotintransf.
+      assert (l1 <> p /\ ~ Dominators.member l1 (DomDS.st_in st)!!p)
+        as J.
+        split; intro J; subst; apply Hnotintransf.
+          apply Dominators.add_member1; auto.
+          apply Dominators.add_member2; auto.
+      clear Hnotintransf.
+      destruct J as [Hneq J].
+      apply Hdom in J; auto.
+      destruct J as [vl [al [J1 J2]]].
+      exists (index p::vl). exists (A_ends (index l2) (index p)::al).
+      split.
+      SSCase "1".
+        apply XATree.make_predecessors_correct' in Hinpds.
+        change (successors_blocks bs) with (successors (fdef_intro fh bs))
+          in Hinpds.
+        apply successors__blockInFdefB in Hinpds.
+        destruct Hinpds as [ps0 [cs0 [tmn0 [J3 J4]]]].
+        constructor; eauto.
+          eapply successor_in_arcs; eauto.
+
+      SSCase "2".
+          intro J. simpl in J.
+          destruct J as [J | J]; auto.
+            inv J. auto.
+  Case "n<>l2".
+    rewrite J2 in H0; auto.
+Qed.
+
+Lemma propagate_succ_list_non_sdomination_aux:
+  forall p scs st out,
+  (forall s, In s scs -> In p predecessors!!!s) ->
+  non_sdomination_prop st.(DomDS.st_in) ->
+  Dominators.ge (transf p st.(DomDS.st_in)!!p) out ->
+  non_sdomination_prop (DomDS.propagate_succ_list st out scs).(DomDS.st_in).
+Proof.
+  induction scs; simpl; intros; auto.
+    apply IHscs; auto.
+      eapply propagate_succ_non_sdomination; eauto.
+      apply Dominators.ge_trans with (y:=transf p (DomDS.st_in st) !! p);
+        auto.
+        eapply EntryDomsOthers.transf_mono; eauto.
+        destruct (@DomDS.propagate_succ_spec st out a) as [J1 J2].
+        destruct (eq_atom_dec a p); subst.
+          apply Dominators.ge_trans with
+            (y:=Dominators.lub (DomDS.st_in st) !! p out).
+            apply Dominators.ge_refl; auto.
+            apply Dominators.ge_lub_left.
+          rewrite J2; auto.
+            apply Dominators.ge_refl'.
+Qed.
+
+Lemma propagate_succ_list_non_sdomination:
+  forall p scs st,
+  (forall s, In s scs -> In p predecessors!!!s) ->
+  non_sdomination_prop st.(DomDS.st_in) ->
+  non_sdomination_prop (DomDS.propagate_succ_list st
+    (transf p st.(DomDS.st_in)!!p) scs).(DomDS.st_in).
+Proof.
+  intros.
+  eapply propagate_succ_list_non_sdomination_aux; eauto.
+    apply Dominators.ge_refl'.
+Qed.
+
+Lemma step_non_sdomination:
+  forall st n rem,
+  AtomNodeSet.pick st.(DomDS.st_wrk) = Some(n, rem) ->
+  non_sdomination_prop st.(DomDS.st_in) ->
+  non_sdomination_prop (DomDS.propagate_succ_list 
+                                 (DomDS.mkstate st.(DomDS.st_in) rem)
+                                 (transf n st.(DomDS.st_in)!!n)
+                                 ((successors_blocks bs)!!!n)).(DomDS.st_in).
+Proof.
+  intros st n rem WKL GOOD.
+  destruct st. simpl.
+  apply propagate_succ_list_non_sdomination; auto.
+    apply XATree.make_predecessors_correct.
+Qed.
+
+Theorem dom_non_sdomination: forall res,
+  DomDS.fixpoint (successors_blocks bs) transf entrypoints = Some res ->
+  non_sdomination_prop res.
+Proof.
+  unfold DomDS.fixpoint. intros res PI. pattern res.
+  eapply (PrimIter.iterate_prop _ _ (DomDS.step _ _)
+    (fun st => non_sdomination_prop st.(DomDS.st_in))); eauto.
+    intros st GOOD. unfold DomDS.step.
+    caseEq (AtomNodeSet.pick st.(DomDS.st_wrk)); auto.
+    intros [n rem] PICK. apply step_non_sdomination; auto.
+
+    apply start_non_sdomination.
+Qed.
+
+End DomComplete. End DomComplete.
+
+Section sdom_is_complete.
+
+Variable f:fdef.
+
+Hypothesis Hwf_entrypoints: wf_entrypoints f.
+
+Hypothesis branches_in_vertexes: forall p ps0 cs0 tmn0 l2
+  (J3 : blockInFdefB (block_intro p ps0 cs0 tmn0) f)
+  (J4 : In l2 (successors_terminator tmn0)),
+  vertexes_fdef f (index l2).
+
+Lemma sdom_is_complete: forall
+  (l3 : l) (l' : l) ps cs tmn ps' cs' tmn'
+  (HuniqF : uniqFdef f)
+  (Hsucc: dom_analysis_is_successful f)
+  (HBinF' : blockInFdefB (block_intro l' ps' cs' tmn') f = true)
+  (HBinF : blockInFdefB (block_intro l3 ps cs tmn) f = true)
+  (Hsdom: strict_domination f l' l3),
+  In l' (dom_query f l3).
+Proof.
+  intros. 
+  unfold wf_entrypoints, dom_analysis_is_successful, 
+         dom_query, dom_analyze in *. 
+  destruct f as [fh bs].
+  remember (getEntryBlock (fdef_intro fh bs)) as R.
+  destruct R as [[le ? ? ?] | ]; try tauto.
+  remember (DomDS.fixpoint 
+                  (successors_blocks bs)
+                  transfer
+                  ((le, Dominators.top) :: nil)) as R.
+  destruct R; try tauto.
+      symmetry in HeqR0.
+      eapply DomComplete.dom_non_sdomination with (entry:=le) in HeqR0; eauto.
+      SSCase "1".
+        Focus.
+        unfold DomComplete.non_sdomination_prop in HeqR0.
+        assert (vertexes_fdef (fdef_intro fh bs) (index l')) as J.
+          apply blockInFdefB_in_vertexes in HBinF'; auto.
+        destruct (Dominators.member_dec l' (t!!l3)).
+        SSSCase "1".
+          unfold Dominators.member in H.
+          destruct (t!!l3); auto.
+
+        SSSCase "2".
+          apply HeqR0 with (l2:=l3) in J; auto.
+            unfold DomComplete.non_sdomination in J.
+            destruct J as [vl [al [J1 J2]]].
+            unfold strict_domination in Hsdom.
+            destruct Hsdom as [Hdom Hneq].
+            unfold domination in Hdom.
+            simpl in Hdom.
+            destruct bs as [|[]]; inv HeqR.
+            apply Hdom in J1.
+            destruct J1; subst; congruence.
+        Unfocus.
+
+      SSCase "2".
+        split; auto.
+        split.
+          simpl in *.
+          destruct bs; uniq_result; auto.
+            congruence.
+
+          exists Dominators.top. 
+          split; auto. simpl. apply set_eq_refl.
+Qed.
+
+End sdom_is_complete.
+
+Module UnreachableDoms. Section UnreachableDoms.
+
+Variable fh : fheader.
+Variable bs : blocks.
+Definition predecessors := XATree.make_predecessors (successors_blocks bs).
+Definition transf := transfer.
+Definition top := Dominators.top.
+Definition bot := Dominators.bot.
+Variable entry: l.
+Variable entrypoints: list (atom * DomDS.L.t).
+
+Hypothesis wf_entrypoints:
+  predecessors!!!entry = nil /\
+  match bs with
+  | block_intro l0 _ _ _ :: _ => l0 = entry
+  | _ => False
+  end /\
+  exists v, [(entry, v)] = entrypoints /\ Dominators.eq v top.
+
+Definition unreachable_doms (res: AMap.t DomDS.L.t) : Prop :=
+  forall l0, ~ reachable (fdef_intro fh bs) l0 -> l0 <> entry ->
+  Dominators.eq res!!l0 bot.
+
+Lemma start_unreachable_doms:
+  unreachable_doms
+    (DomDS.st_in (DomDS.start_state (successors_blocks bs) entrypoints)).
+Proof.
+  intros l0 Hunreach Heq.
+  unfold DomDS.start_state. simpl.
+  eapply EntryDomsOthers.dom_nonentry_start_state_in in Heq; eauto.
+Qed.
+
+(** We show that the start state satisfies the invariant, and that
+  the [step] function preserves it. *)
+
+Lemma propagate_succ_unreachable_doms: forall st n out,
+  (~ reachable (fdef_intro fh bs) n -> n <> entry -> 
+   Dominators.eq out bot) ->
+  unreachable_doms st.(DomDS.st_in) ->
+  unreachable_doms (DomDS.propagate_succ st out n).(DomDS.st_in).
+Proof.
+  unfold unreachable_doms.
+  intros.
+  destruct (@DomDS.propagate_succ_spec st out n) as [J1 J2].
+  assert (H':=H1).
+  apply H0 in H1; auto.
+  destruct (eq_atom_dec n l0); subst.
+    apply H in H'; auto.
+    apply Dominators.eq_trans with
+      (y:=DomDS.L.lub (DomDS.st_in st) !! l0 out); auto.
+    apply Dominators.eq_trans with (y:=DomDS.L.lub bot bot); auto.
+       apply Dominators.lub_compat_eq; auto.
+       apply Dominators.eq_sym. apply Dominators.lub_refl.
+
+    rewrite J2; auto.
+Qed.
+
+Lemma propagate_succ_list_unreachable_doms:
+  forall scs st out,
+  (forall s, In s scs ->
+             ~ reachable (fdef_intro fh bs) s -> s <> entry ->
+             Dominators.eq out bot) ->
+  unreachable_doms st.(DomDS.st_in) ->
+  unreachable_doms (DomDS.propagate_succ_list st out scs).(DomDS.st_in).
+Proof.
+  induction scs; simpl; intros; auto.
+    apply IHscs.
+      intros. apply H with (s:=s); auto.
+      apply propagate_succ_unreachable_doms; auto.
+        intros J1 J2. eapply H; eauto.
+Qed.
+
+Hypothesis branches_in_vertexes: forall p ps0 cs0 tmn0 l2
+  (J3 : blockInFdefB (block_intro p ps0 cs0 tmn0) (fdef_intro fh bs))
+  (J4 : In l2 (successors_terminator tmn0)),
+  vertexes_fdef (fdef_intro fh bs) (index l2).
+
+Hypothesis UniqF: uniqFdef (fdef_intro fh bs).
+
+Lemma step_unreachable_doms:
+  forall st n rem,
+  AtomNodeSet.pick st.(DomDS.st_wrk) = Some(n, rem) ->
+  unreachable_doms st.(DomDS.st_in) ->
+  unreachable_doms (DomDS.propagate_succ_list 
+                                  (DomDS.mkstate st.(DomDS.st_in) rem)
+                                  (transf n st.(DomDS.st_in)!!n)
+                                  ((successors_blocks bs)!!!n)).(DomDS.st_in).
+Proof.
+  intros st n rem WKL GOOD.
+  destruct st. simpl.
+  apply propagate_succ_list_unreachable_doms; auto.
+  intros s Hin Hunreach.
+    destruct (reachable_dec (fdef_intro fh bs) n).
+    Case "reach".
+      assert(exists ps0, exists cs0, exists tmn0,
+        blockInFdefB (block_intro n ps0 cs0 tmn0) (fdef_intro fh bs) /\
+        In s (successors_terminator tmn0)) as J.
+        apply successors__blockInFdefB; auto.
+      destruct J as [ps0 [cs0 [tmn0 [J1 J2]]]].
+      eapply DecRD.reachable_successors with (l1:=s) in H; eauto.
+        congruence.
+
+    Case "unreach".
+      apply GOOD in H. simpl in H.
+      unfold transf, transfer.
+      intros.
+      destruct (eq_atom_dec n entry); subst.
+        assert (exists ps0, exists cs0, exists tmn0,
+          blockInFdefB (block_intro entry ps0 cs0 tmn0) (fdef_intro fh bs) /\
+          In s (successors_terminator tmn0)) as J.
+          apply successors__blockInFdefB; auto.
+        destruct J as [ps0 [cs0 [tmn0 [J1 J2]]]].
+        contradict Hunreach.
+        unfold reachable. 
+        destruct wf_entrypoints as [_ [J _]].
+        destruct bs as [|b ?]; tinv J. 
+        destruct b as [l5 ? ? ?]. simpl. subst entry.
+        unfold XATree.successors_list in Hin. simpl in Hin. rewrite ATree.gss in Hin.
+        clear J.
+        exists (index l5::nil). exists (A_ends (index s) (index l5)::nil).
+        constructor; eauto.
+          constructor.
+            eapply entry_in_vertexes; simpl; eauto.
+          eapply successor_in_arcs; eauto.
+      apply Dominators.eq_trans with (y:=Dominators.add (Dominators.bot) n).
+        apply Dominators.add_eq; auto.
+        apply Dominators.add_bot.
+Qed.
+
+Theorem dom_unreachable_doms: forall res,
+  DomDS.fixpoint (successors_blocks bs) transf entrypoints = Some res ->
+  unreachable_doms res.
+Proof.
+  unfold DomDS.fixpoint. intros res PI. pattern res.
+  eapply (PrimIter.iterate_prop _ _ (DomDS.step _ _)
+    (fun st => unreachable_doms st.(DomDS.st_in))); eauto.
+  intros st GOOD. unfold DomDS.step.
+  caseEq (AtomNodeSet.pick st.(DomDS.st_wrk)); auto.
+  intros [n rem] PICK.
+  apply step_unreachable_doms; auto.
+    apply start_unreachable_doms.
+Qed.
+
+End UnreachableDoms. End UnreachableDoms. 
+
+Section dom_unreachable.
+
+Variable f:fdef.
+
+Hypothesis branches_in_vertexes: forall p ps0 cs0 tmn0 l2
+  (J3 : blockInFdefB (block_intro p ps0 cs0 tmn0) f)
+  (J4 : In l2 (successors_terminator tmn0)),
+  vertexes_fdef f (index l2).
+
+Hypothesis wf_entrypoints:
+  match getEntryBlock f with
+  | Some (block_intro l0 _ _ _) => 
+      (XATree.make_predecessors (successors f))!!!l0 = nil
+  | _ => False
+  end.
+
+Lemma dom_unreachable: forall
+  (l3 : l) (l' : l) ps cs tmn
+  (Hsucc: dom_analysis_is_successful f)
+  (HuniqF: uniqFdef f)
+  (HBinF : blockInFdefB (block_intro l3 ps cs tmn) f = true)
+  (Hunreach: ~ reachable f l3),
+  dom_query f l3 = bound_fdef f.
+Proof.
+  intros.
+  case_eq (getEntryBlock f); 
+    try solve [intros EQ; rewrite EQ in wf_entrypoints; tauto].
+  intros [l0 p c t] Hentry. 
+  match goal with | H1: getEntryBlock _ = _ |- _ =>
+    assert (J:=H1); apply dom_entrypoint in H1 end.
+  destruct f as [fh bs].
+  destruct (id_dec l3 l0); subst.
+  Case "l3=l0".
+    contradict Hunreach.
+    eapply reachable_entrypoint; eauto.
+  Case "l3<>l0".
+    unfold dom_query, dom_analyze, dom_analysis_is_successful in *.
+    match goal with | H1: getEntryBlock _ = _ |- _ => rewrite H1 in * end.
+    remember (DomDS.fixpoint 
+                  (successors_blocks bs)
+                  transfer
+                  ((l0, Dominators.top) :: nil)) as R.
+    destruct R; try tauto.
+      symmetry in HeqR.
+      eapply UnreachableDoms.dom_unreachable_doms with (entry:=l0) in HeqR;
+        eauto.
+      SCase "1".
+        apply HeqR in n; auto.
+        simpl. destruct t0 !! l3; tinv n. auto.
+      SCase "2".
+        split; auto.
+        split.
+          simpl in J.
+          destruct bs; uniq_result; auto.
+
+          exists Dominators.top. 
+          split; auto. simpl. apply set_eq_refl.
+Qed.
+
+End dom_unreachable.
+
+Section sound_acyclic.
+
+Variable f : fdef.
+Hypothesis Hhasentry: getEntryBlock f <> None.
+
+Lemma dom_is_sound : forall
+  (l3 : l) (l' : l) ps cs tmn
+  (HBinF : blockInFdefB (block_intro l3 ps cs tmn) f = true)
+  (Hin : In l' (l3::(dom_query f l3))),
+  domination f l' l3.
+Proof.
+  unfold domination, strict_domination.
+  intros. destruct f as [fh bs].
+  remember (getEntryBlock (fdef_intro fh bs)) as R.
+  destruct R; try congruence. clear Hhasentry.
+  destruct b as [l5 ps5 cs5 t5].
+  intros vl al Hreach.
+  generalize dependent ps.
+  generalize dependent cs.
+  generalize dependent tmn.
+  remember (vertexes_fdef (fdef_intro fh bs)) as Vs.
+  remember (arcs_fdef (fdef_intro fh bs)) as As.
+  remember (index l3) as v0.
+  remember (index l5) as v1.
+  generalize dependent bs.
+  generalize dependent l3.
+  generalize dependent l5.
+  induction Hreach; intros; subst.
+    inv Heqv0. symmetry in HeqR.
+    apply dom_entrypoint in HeqR.
+    rewrite HeqR in Hin.
+    simpl in Hin. destruct Hin as [Hin | Hin]; tinv Hin; auto.
+
+    destruct y as [a0].
+    assert (exists ps0, exists cs0, exists tmn0,
+      blockInFdefB (block_intro a0 ps0 cs0 tmn0) (fdef_intro fh bs) /\
+      In l3 (successors_terminator tmn0)) as J.
+      eapply successors__blockInFdefB; eauto.
+    destruct J as [ps0 [cs0 [tmn0 [HBinF'' Hinsucc]]]].
+    remember ((dom_analyze (fdef_intro fh bs)) !! a0) as R0.
+    destruct (id_dec l' l3); subst; auto.
+    left.
+    assert (In l'
+      (a0 :: (dom_query (fdef_intro fh bs) a0))) as J.
+      assert (incl (dom_query (fdef_intro fh bs) l3)
+                   (a0 :: (dom_query (fdef_intro fh bs) a0))) as Hinc.
+        eapply dom_successors; eauto.
+      simpl in Hin. destruct Hin; try congruence.
+      apply Hinc; auto.
+    eapply IHHreach in J; eauto.
+    simpl.
+    destruct J as [J | J]; subst; eauto.
+Qed.
+
+Lemma sdom_is_sound : forall
+  (l3 : l) (l' : l) ps cs tmn
+  (Hreach : reachable f l3)
+  (HBinF : blockInFdefB (block_intro l3 ps cs tmn) f = true)
+  (Hin : In l' (dom_query f l3)),
+  strict_domination f l' l3.
+Proof. 
+  intros.
+  eapply dom_is_sound with (l':=l') in HBinF; simpl; eauto.
+  split; auto.
+  destruct (id_dec l' l3); subst; auto.
+  unfold reachable, domination in *.
+  remember (getEntryBlock f) as R.
+  destruct R; try congruence.
+  destruct b as [l0 ? ? ?].
+  destruct Hreach as [vl [al Hreach]].
+  apply DWalk_to_dpath in Hreach; auto.
+  destruct Hreach as [vl0 [al0 Hp]].
+  destruct (id_dec l3 l0); subst.
+    symmetry in HeqR.
+    apply dom_entrypoint in HeqR.
+    rewrite HeqR in Hin. inv Hin.
+
+    inv Hp; try congruence.
+    destruct y as [a0].
+    assert (exists ps0, exists cs0, exists tmn0,
+      blockInFdefB (block_intro a0 ps0 cs0 tmn0) f /\
+      In l3 (successors_terminator tmn0)) as J.
+      eapply successors__blockInFdefB; eauto.
+    destruct J as [ps0 [cs0 [tmn0 [HBinF' Hinsucc]]]].
+    remember ((dom_analyze f) !! a0) as R0.
+   assert (In l3 (a0 :: (dom_query f a0))) as J.
+      assert (incl (dom_query f l3) (a0 :: (dom_query f a0))) as Hinc.
+        destruct f. eapply dom_successors; eauto.
+      simpl in Hin.
+      apply Hinc; auto.
+    eapply dom_is_sound in J; eauto.
+    unfold domination in J.
+    rewrite <- HeqR in J.
+    assert (Hw:=H).
+    apply D_path_isa_walk in Hw.
+    apply J in Hw.
+    destruct Hw as [Hw | Hw]; subst; auto.
+      apply H4 in Hw. inv Hw; try congruence.
+Qed.
+
+Lemma sdom_isnt_refl : forall
+  (l3 : l) (l' : l) ps cs tmn
+  (Hreach : reachable f l3)
+  (HBinF : blockInFdefB (block_intro l3 ps cs tmn) f = true)
+  (Hin : In l' (dom_query f l3)),
+  l' <> l3.
+Proof. 
+  intros.
+  eapply sdom_is_sound in Hin; eauto.
+  destruct Hin; auto.
+Qed.
+
+Definition getEntryBlock_inv f := forall
+  (l3 : l)
+  (l' : l)
+  (ps : phinodes)
+  (cs : cmds)
+  (tmn : terminator)
+  (HBinF : blockInFdefB (block_intro l3 ps cs tmn) f = true)
+  (Hsucc : In l' (successors_terminator tmn)) a ps0 cs0 tmn0
+  (H : getEntryBlock f = Some (block_intro a ps0 cs0 tmn0)),
+  l' <> a.
+
+Lemma adom_acyclic: forall 
+  (HgetEntryBlock_inv : getEntryBlock_inv f)
+  l1 l2 ps1 cs1 tmn1 ps2 cs2 tmn2,
+  reachable f l2 ->
+  blockInFdefB (block_intro l1 ps1 cs1 tmn1) f = true ->
+  blockInFdefB (block_intro l2 ps2 cs2 tmn2) f = true ->
+  In l1 (dom_query f l2) ->
+  In l2 (dom_query f l1) ->
+  l1 <> l2 ->
+  False.
+Proof.
+  intros.
+  assert (strict_domination f l1 l2) as Hdom12.
+    eapply sdom_is_sound; eauto.
+  assert (strict_domination f l2 l1) as Hdom21.
+    eapply sdom_is_sound; eauto.
+      apply DecDom.sdom_reachable in Hdom12; auto.
+  eapply DecDom.dom_acyclic in Hdom12; eauto.
+  apply Hdom12. destruct Hdom21; auto.
+Qed.
+
+End sound_acyclic.
+
+Section pres_dom.
+
+Variable ftrans: fdef -> fdef.
+Variable btrans: block -> block.
+
+Hypothesis ftrans_spec: forall fh bs, 
+  ftrans (fdef_intro fh bs) = fdef_intro fh (List.map btrans bs).
+
+Hypothesis btrans_eq_label: forall b, getBlockLabel b = getBlockLabel (btrans b).
+
+Lemma pres_getEntryBlock : forall f b
+  (Hentry : getEntryBlock f = Some b),
+  getEntryBlock (ftrans f) = Some (btrans b).
+Proof.
+  intros. destruct f as [fh bs]. rewrite ftrans_spec.
+  destruct bs; inv Hentry; auto.
+Qed.
+
+Lemma pres_getEntryBlock_None : forall f
+  (Hentry : getEntryBlock f = None),
+  getEntryBlock (ftrans f) = None.
+Proof.
+  intros. destruct f as [fh bs]. rewrite ftrans_spec.
+  destruct bs; inv Hentry; auto.
+Qed.
+
+Lemma pres_bound_blocks : forall bs,
+  bound_blocks bs = bound_blocks (List.map btrans bs).
+Proof.
+  induction bs as [|a bs]; simpl; auto.
+    assert (J:=btrans_eq_label a);
+    remember (btrans a) as R.
+    destruct R as [l1 ? ? ?]; destruct a; simpl in *; subst l1.
+    congruence.
+Qed.
+
+Hypothesis btrans_eq_tmn: forall b, 
+  terminator_match (getBlockTmn b) (getBlockTmn (btrans b)).
+
+Lemma pres_successors_blocks : forall bs,
+  successors_blocks bs = successors_blocks (List.map btrans bs).
+Proof.
+  induction bs as [|b bs]; simpl; auto.
+    assert (J:=btrans_eq_tmn b).
+    assert (J':=btrans_eq_label b).
+    remember (btrans b) as R.
+    destruct R as [l1 ? ? ?]; destruct b; simpl in *; subst l1.
+    rewrite IHbs. 
+    terminator_match_tac.
+Qed.
+
+Lemma pres_dom_query: forall (f : fdef) (l5 l0 : l),
+  ListSet.set_In l5 (AlgDom.dom_query f l0) <->
+  ListSet.set_In l5 (AlgDom.dom_query (ftrans f) l0).
+Proof.
+  intros.
+  unfold AlgDom.dom_query, AlgDom.dom_analyze. destruct f as [fh bs]. 
+  case_eq (getEntryBlock (fdef_intro fh bs)).
+    intros b Hentry.
+    apply pres_getEntryBlock in Hentry; eauto.
+    assert (J:=btrans_eq_label b);
+    remember (btrans b) as R.
+    destruct R as [l1 ? ? ?]; destruct b; simpl in *; subst l1.
+    rewrite Hentry. rewrite ftrans_spec. simpl.
+    rewrite <- pres_bound_blocks.
+    rewrite <- pres_successors_blocks. split; eauto.
+
+    intros Hentry.
+    apply pres_getEntryBlock_None in Hentry; eauto.
+    rewrite Hentry. rewrite ftrans_spec. simpl.
+    rewrite <- pres_bound_blocks. split; auto.
+Qed.
+
+Lemma pres_dom_analysis_is_successful : forall f,
+  AlgDom.dom_analysis_is_successful f <-> 
+    AlgDom.dom_analysis_is_successful (ftrans f).
+Proof.
+  unfold AlgDom.dom_analysis_is_successful.
+  destruct f as [fh bs]. 
+  case_eq (getEntryBlock (fdef_intro fh bs)).
+    intros b Hentry.
+    apply pres_getEntryBlock in Hentry; eauto.
+    assert (J:=btrans_eq_label b);
+    remember (btrans b) as R.
+    destruct R as [l1 ? ? ?]; destruct b; simpl in *; subst l1.
+    rewrite Hentry. rewrite ftrans_spec. simpl.
+    rewrite <- pres_successors_blocks. split; eauto.
+
+    intros Hentry.
+    apply pres_getEntryBlock_None in Hentry; eauto.
+    rewrite Hentry. rewrite ftrans_spec. simpl.
+    split; auto.
+Qed.
+
+End pres_dom.
+
+End AlgDom.
