src3.0/Vellvm/Dominators/reach.v
@@ -1,0 +1,56 @@
+Require Import List.
+Require Import ListSet.
+Require Import Coqlib.
+Require Import Metatheory.
+Require Import Maps.
+Require Import cfg.
+Require Import Dipaths.
+
+Require Import syntax.
+Require Import infrastructure.
+Require Import infrastructure_props.
+Import LLVMsyntax.
+Import LLVMinfra.
+
+Lemma reachable_dec: forall (f:fdef) (l1:l), reachable f l1 \/ ~ reachable f l1.
+Proof. intros. tauto. Qed. (* classic logic *)
+
+Lemma reachable_entrypoint:
+  forall (f:fdef) l0 ps cs tmn,
+    getEntryBlock f = Some (block_intro l0 ps cs tmn) ->
+    reachable f l0.
+Proof.
+  intros f l0 ps cs tmn Hentry. unfold reachable.
+  rewrite Hentry. exists V_nil. exists A_nil. apply DW_null.
+  eapply entry_in_vertexes; eauto.
+Qed.
+
+Module DecRD.
+
+Section RdSucc.
+
+Variable f:fdef.
+
+Lemma reachable_successors:
+  forall l0 cs ps tmn l1 (Hinvx: vertexes_fdef f (index l1)),
+  uniqFdef f -> 
+  blockInFdefB (block_intro l0 cs ps tmn) f ->
+  In l1 (successors_terminator tmn) ->
+  reachable f l0 ->
+  reachable f l1.
+Proof.
+  intros l0 cs ps tmn l1 Hinvx HuniqF HbInF Hin.
+  unfold reachable. intro Hreach.
+  remember (getEntryBlock f) as R.
+  destruct R; auto.
+  destruct b as [le ? ? ?].
+  destruct Hreach as [vl [al Hreach]].
+  exists (index l0::vl). exists (A_ends (index l1) (index l0)::al).
+  apply DW_step; auto.
+    eapply successor_in_arcs; eauto.
+Qed.
+
+End RdSucc.
+
+End DecRD.
+
