src3.0/Vellvm/opsem_dom.v
@@ -2,6 +2,7 @@ Require Import Ensembles.
 Require Import syntax.
 Require Import infrastructure.
 Require Import infrastructure_props.
+Require Import dom_set.
 Require Import analysis.
 Require Import typings.
 Require Import typings_props.
@@ -250,7 +251,7 @@ Lemma wf_defs_br_aux : forall TD gl S M lc l' ps' cs' lc' F tmn' b
   (ids0' : list atom)
   (HwfF : wf_fdef S M F) (HuniqF: uniqFdef F)
   (contents' : ListSet.set atom)
-  (Heqdefs' : contents' = dom_query F l')
+  (Heqdefs' : contents' = AlgDom.dom_query F l')
   (Hinscope : (fold_left (inscope_of_block F l') contents'
     (ret (getPhiNodesIDs ps' ++ getArgsIDsOfFdef F)) = ret ids0'))
   (Hinc : incl (ListSet.set_diff eq_atom_dec ids0' (getPhiNodesIDs ps')) t),
@@ -320,8 +321,8 @@ Proof.
   unfold inscope_of_tmn. unfold inscope_of_cmd, inscope_of_id.
   destruct F as [fh bs].
 
-  assert (incl (dom_query (fdef_intro fh bs) l')
-    (l3::(dom_query (fdef_intro fh bs) l3))) as Hsub.
+  assert (incl (AlgDom.dom_query (fdef_intro fh bs) l')
+    (l3::(AlgDom.dom_query (fdef_intro fh bs) l3))) as Hsub.
     clear - HBinF Hsucc HuniqF HwfF.
     eapply dom_successors; eauto.
 
@@ -329,7 +330,7 @@ Proof.
     as Hreach'.
     eapply isReachableFromEntry_successors in Hlkup; eauto.
 
-  assert (J1:=dom_query_in_bound fh bs l').
+  assert (J1:=AlgDom.dom_query_in_bound fh bs l').
   destruct fh as [f t i0 a v].
   apply fold_left__bound_blocks with (init:=getPhiNodesIDs ps' ++
       getCmdsIDs nil ++ getArgsIDs a)(bs:=bs)(l0:=l')
@@ -1785,7 +1786,7 @@ Case "sCall".
       assert (ps'=nil) as EQ.
         eapply entryBlock_has_no_phinodes with (s:=S); eauto.        
       subst.
-      apply dom_entrypoint in H2.
+      apply AlgDom.dom_entrypoint in H2.
       destruct cs'.
         unfold inscope_of_tmn.
         rewrite H2. simpl.
